<?xml version="1.0" encoding="UTF-8"?><rdf:RDF
    xml:base="http://rdaregistry.info/Elements/p/"
    xmlns:dc="http://purl.org/dc/elements/1.1/"
    xmlns:foaf="http://xmlns.com/foaf/0.1/"
    xmlns:rdakit="http://metadataregistry.org/uri/profile/rdakit/"
    xmlns:rdf="http://www.w3.org/1999/02/22-rdf-syntax-ns#"
    xmlns:rdfs="http://www.w3.org/2000/01/rdf-schema#"
    xmlns:reg="http://metadataregistry.org/uri/profile/regap/"
    xmlns:skos="http://www.w3.org/2004/02/skos/core#">

<!-- Element Set: RDA Place properties -->
<rdf:Description rdf:about="http://rdaregistry.info/Elements/p/">
  <dc:title xml:lang="en">RDA Place properties</dc:title>
  <skos:note  xml:lang="en">Properties derived from RDA elements with the domain of RDA Place.</skos:note>
</rdf:Description>

<!-- Properties -->

<!-- Property: has access point for place -->
<rdf:Description rdf:about="http://rdaregistry.info/Elements/p/P70018">
  <rdfs:isDefinedBy rdf:resource="http://rdaregistry.info/Elements/p/" />
  <reg:status rdf:resource="http://metadataregistry.org/uri/RegStatus/1001" />
  <rdf:type rdf:resource="http://www.w3.org/1999/02/22-rdf-syntax-ns#Property" />
  <reg:name xml:lang="en">accessPointForPlace</reg:name>
  <rdfs:label xml:lang="en">has access point for place</rdfs:label>
  <reg:lexicalAlias rdf:resource="http://rdaregistry.info/Elements/p/accessPointForPlace.en" />
  <skos:definition xml:lang="en">Relates a place to an appellation of place in natural language that is taken from a vocabulary encoding scheme or is constructed using a string encoding scheme.</skos:definition>
  <rdfs:domain rdf:resource="http://rdaregistry.info/Elements/c/C10009" />
  <rdakit:toolkitLabel xml:lang="en">access point for place</rdakit:toolkitLabel>
  <rdakit:toolkitDefinition xml:lang="en">An appellation of place in natural language that is taken from a vocabulary encoding scheme or is constructed using a string encoding scheme.</rdakit:toolkitDefinition>
  <reg:hasUnconstrained rdf:resource="http://rdaregistry.info/Elements/u/P60906" />
  <reg:hasSubproperty rdf:resource="http://rdaregistry.info/Elements/p/object/P70018" />
  <rdfs:subPropertyOf rdf:resource="http://rdaregistry.info/Elements/p/P70019" />
  <rdakit:hasElementType xml:lang="">3</rdakit:hasElementType>
  <reg:hasSubproperty rdf:resource="http://rdaregistry.info/Elements/p/datatype/P70018" />
  <reg:hasSubproperty rdf:resource="http://rdaregistry.info/Elements/p/P70045" />
  <reg:hasSubproperty rdf:resource="http://rdaregistry.info/Elements/p/P70046" />
  <rdfs:subPropertyOf rdf:resource="http://rdaregistry.info/Elements/x/P00016" />
</rdf:Description>

<!-- Property: has appellation of place -->
<rdf:Description rdf:about="http://rdaregistry.info/Elements/p/P70019">
  <rdfs:isDefinedBy rdf:resource="http://rdaregistry.info/Elements/p/" />
  <reg:status rdf:resource="http://metadataregistry.org/uri/RegStatus/1001" />
  <rdf:type rdf:resource="http://www.w3.org/1999/02/22-rdf-syntax-ns#Property" />
  <reg:name xml:lang="en">appellationOfPlace</reg:name>
  <rdfs:label xml:lang="en">has appellation of place</rdfs:label>
  <reg:lexicalAlias rdf:resource="http://rdaregistry.info/Elements/p/appellationOfPlace.en" />
  <skos:definition xml:lang="en">Relates a place to a nomen used within a given scheme or context to refer to a place.</skos:definition>
  <rdfs:domain rdf:resource="http://rdaregistry.info/Elements/c/C10009" />
  <rdakit:toolkitLabel xml:lang="en">appellation of place</rdakit:toolkitLabel>
  <rdakit:toolkitDefinition xml:lang="en">A nomen used within a given scheme or context to refer to a place.</rdakit:toolkitDefinition>
  <reg:hasSubproperty rdf:resource="http://rdaregistry.info/Elements/p/P70001" />
  <reg:hasUnconstrained rdf:resource="http://rdaregistry.info/Elements/u/P60909" />
  <reg:hasSubproperty rdf:resource="http://rdaregistry.info/Elements/p/object/P70019" />
  <rdfs:subPropertyOf rdf:resource="http://rdaregistry.info/Elements/p/P70012" />
  <rdakit:hasElementType xml:lang="">3</rdakit:hasElementType>
  <reg:hasSubproperty rdf:resource="http://rdaregistry.info/Elements/p/datatype/P70019" />
  <reg:hasSubproperty rdf:resource="http://rdaregistry.info/Elements/p/P70018" />
  <reg:hasSubproperty rdf:resource="http://rdaregistry.info/Elements/p/P70020" />
  <rdfs:subPropertyOf rdf:resource="http://rdaregistry.info/Elements/x/P00017" />
</rdf:Description>

<!-- Property: has authorized access point for place -->
<rdf:Description rdf:about="http://rdaregistry.info/Elements/p/P70045">
  <rdfs:isDefinedBy rdf:resource="http://rdaregistry.info/Elements/p/" />
  <reg:status rdf:resource="http://metadataregistry.org/uri/RegStatus/1001" />
  <rdf:type rdf:resource="http://www.w3.org/1999/02/22-rdf-syntax-ns#Property" />
  <reg:name xml:lang="en">authorizedAccessPointForPlace</reg:name>
  <rdfs:label xml:lang="en">has authorized access point for place</rdfs:label>
  <reg:lexicalAlias rdf:resource="http://rdaregistry.info/Elements/p/authorizedAccessPointForPlace.en" />
  <skos:definition xml:lang="en">Relates a place to an access point of place that is selected for preference in a specific vocabulary encoding scheme.</skos:definition>
  <rdfs:domain rdf:resource="http://rdaregistry.info/Elements/c/C10009" />
  <rdakit:toolkitLabel xml:lang="en">authorized access point for place</rdakit:toolkitLabel>
  <rdakit:toolkitDefinition xml:lang="en">An access point of place that is selected for preference in a specific vocabulary encoding scheme.</rdakit:toolkitDefinition>
  <reg:hasUnconstrained rdf:resource="http://rdaregistry.info/Elements/u/P60916" />
  <reg:hasSubproperty rdf:resource="http://rdaregistry.info/Elements/p/object/P70045" />
  <rdfs:subPropertyOf rdf:resource="http://rdaregistry.info/Elements/p/P70018" />
  <rdakit:hasElementType xml:lang="">3</rdakit:hasElementType>
  <reg:hasSubproperty rdf:resource="http://rdaregistry.info/Elements/p/datatype/P70045" />
  <rdfs:subPropertyOf rdf:resource="http://rdaregistry.info/Elements/x/P00020" />
</rdf:Description>

<!-- Property: has category of place -->
<rdf:Description rdf:about="http://rdaregistry.info/Elements/p/P70044">
  <rdfs:isDefinedBy rdf:resource="http://rdaregistry.info/Elements/p/" />
  <reg:status rdf:resource="http://metadataregistry.org/uri/RegStatus/1001" />
  <rdf:type rdf:resource="http://www.w3.org/1999/02/22-rdf-syntax-ns#Property" />
  <reg:name xml:lang="en">categoryOfPlace</reg:name>
  <rdfs:label xml:lang="en">has category of place</rdfs:label>
  <reg:lexicalAlias rdf:resource="http://rdaregistry.info/Elements/p/categoryOfPlace.en" />
  <skos:definition xml:lang="en">Relates a place to a type to which a place belongs.</skos:definition>
  <rdfs:domain rdf:resource="http://rdaregistry.info/Elements/c/C10009" />
  <rdakit:toolkitLabel xml:lang="en">category of place</rdakit:toolkitLabel>
  <rdakit:toolkitDefinition xml:lang="en">A type to which a place belongs.</rdakit:toolkitDefinition>
  <reg:hasUnconstrained rdf:resource="http://rdaregistry.info/Elements/u/P60944" />
  <rdakit:hasElementType xml:lang="">5</rdakit:hasElementType>
  <reg:hasSubproperty rdf:resource="http://rdaregistry.info/Elements/p/datatype/P70044" />
  <skos:altLabel xml:lang="en">type of place</skos:altLabel>
  <rdfs:subPropertyOf rdf:resource="http://rdaregistry.info/Elements/x/P00029" />
</rdf:Description>

<!-- Property: is coordinates of cartographic content of -->
<rdf:Description rdf:about="http://rdaregistry.info/Elements/p/P70023">
  <rdfs:isDefinedBy rdf:resource="http://rdaregistry.info/Elements/p/" />
  <reg:status rdf:resource="http://metadataregistry.org/uri/RegStatus/1001" />
  <rdf:type rdf:resource="http://www.w3.org/1999/02/22-rdf-syntax-ns#Property" />
  <reg:name xml:lang="en">coordinatesOfCartographicContentOf</reg:name>
  <rdfs:label xml:lang="en">is coordinates of cartographic content of</rdfs:label>
  <reg:lexicalAlias rdf:resource="http://rdaregistry.info/Elements/p/coordinatesOfCartographicContentOf.en" />
  <rdfs:domain rdf:resource="http://rdaregistry.info/Elements/c/C10009" />
  <rdakit:toolkitLabel xml:lang="en">coordinates of cartographic content of</rdakit:toolkitLabel>
  <reg:hasSubproperty rdf:resource="http://rdaregistry.info/Elements/p/object/P70023" />
  <rdfs:subPropertyOf rdf:resource="http://rdaregistry.info/Elements/p/P70004" />
  <rdakit:hasElementType xml:lang="">2</rdakit:hasElementType>
  <reg:hasSubproperty rdf:resource="http://rdaregistry.info/Elements/p/datatype/P70023" />
  <skos:definition xml:lang="en">Relates a place to a work that is a cartographic work that has an area of coverage that is described using a mathematical system to identify its boundaries or location.</skos:definition>
  <rdakit:toolkitDefinition xml:lang="en">A work that is a cartographic work that has an area of coverage that is described using a mathematical system to identify its boundaries or location.</rdakit:toolkitDefinition>
  <reg:hasSubproperty rdf:resource="http://rdaregistry.info/Elements/p/P70034" />
  <reg:hasSubproperty rdf:resource="http://rdaregistry.info/Elements/p/P70036" />
  <reg:hasSubproperty rdf:resource="http://rdaregistry.info/Elements/p/P70037" />
</rdf:Description>

<!-- Property: is country associated with person of -->
<rdf:Description rdf:about="http://rdaregistry.info/Elements/p/P70024">
  <rdfs:isDefinedBy rdf:resource="http://rdaregistry.info/Elements/p/" />
  <reg:status rdf:resource="http://metadataregistry.org/uri/RegStatus/1001" />
  <rdf:type rdf:resource="http://www.w3.org/1999/02/22-rdf-syntax-ns#Property" />
  <reg:name xml:lang="en">countryAssociatedWithPersonOf</reg:name>
  <rdfs:label xml:lang="en">is country associated with person of</rdfs:label>
  <reg:lexicalAlias rdf:resource="http://rdaregistry.info/Elements/p/countryAssociatedWithPersonOf.en" />
  <rdfs:domain rdf:resource="http://rdaregistry.info/Elements/c/C10009" />
  <rdakit:toolkitLabel xml:lang="en">country associated with person of</rdakit:toolkitLabel>
  <reg:hasSubproperty rdf:resource="http://rdaregistry.info/Elements/p/object/P70024" />
  <rdfs:subPropertyOf rdf:resource="http://rdaregistry.info/Elements/p/P70014" />
  <rdakit:hasElementType xml:lang="">2</rdakit:hasElementType>
  <skos:definition xml:lang="en">Relates a place to a person who is identified with a country.</skos:definition>
  <rdakit:toolkitDefinition xml:lang="en">A person who is identified with a country.</rdakit:toolkitDefinition>
  <reg:hasUnconstrained rdf:resource="http://rdaregistry.info/Elements/u/P60993" />
  <reg:hasSubproperty rdf:resource="http://rdaregistry.info/Elements/p/datatype/P70024" />
</rdf:Description>

<!-- Property: has name of place -->
<rdf:Description rdf:about="http://rdaregistry.info/Elements/p/P70001">
  <rdfs:isDefinedBy rdf:resource="http://rdaregistry.info/Elements/p/" />
  <reg:status rdf:resource="http://metadataregistry.org/uri/RegStatus/1001" />
  <rdfs:label xml:lang="en">has name of place</rdfs:label>
  <rdf:type rdf:resource="http://www.w3.org/1999/02/22-rdf-syntax-ns#Property" />
  <reg:name xml:lang="en">nameOfPlace</reg:name>
  <skos:definition xml:lang="en">Relates a place to an appellation of place in natural language and phrasing used in common discourse.</skos:definition>
  <rdfs:domain rdf:resource="http://rdaregistry.info/Elements/c/C10009" />
  <reg:lexicalAlias rdf:resource="http://rdaregistry.info/Elements/p/nameOfPlace.en" />
  <rdakit:toolkitLabel xml:lang="en">name of place</rdakit:toolkitLabel>
  <rdakit:toolkitDefinition xml:lang="en">An appellation of place in natural language and phrasing used in common discourse.</rdakit:toolkitDefinition>
  <reg:hasUnconstrained rdf:resource="http://rdaregistry.info/Elements/u/P60366" />
  <rdakit:instructionNumber xml:lang="">16.2</rdakit:instructionNumber>
  <reg:hasSubproperty rdf:resource="http://rdaregistry.info/Elements/p/datatype/P70001" />
  <reg:name xml:lang="da">navnPåEtSted</reg:name>
  <rdfs:label xml:lang="da">har navn på et sted</rdfs:label>
  <reg:lexicalAlias rdf:resource="http://rdaregistry.info/Elements/p/navnPåEtSted.da" />
  <skos:definition xml:lang="da">Relaterer et sted til et ord, tegn eller gruppe af ord og/eller tegn, som et sted er kendt under.</skos:definition>
  <rdakit:toolkitLabel xml:lang="da">navn på et sted</rdakit:toolkitLabel>
  <rdakit:toolkitDefinition xml:lang="da">Ord, tegn eller gruppe af ord og/eller tegn, som et sted er kendt under.</rdakit:toolkitDefinition>
  <reg:name xml:lang="vi">tênĐịaĐiểm</reg:name>
  <rdfs:label xml:lang="vi">có tên địa điểm</rdfs:label>
  <skos:definition xml:lang="vi">Liên kết địa điểm với từ, ký tự, hoặc nhóm từ và/hoặc ký tự mà theo đó địa điểm được biết đến.</skos:definition>
  <rdakit:toolkitLabel xml:lang="vi">tên địa điểm</rdakit:toolkitLabel>
  <rdakit:toolkitDefinition xml:lang="vi">Từ, ký tự, hoặc nhóm từ hoặc ký tự mà theo đó địa điểm được biết đến.</rdakit:toolkitDefinition>
  <rdfs:label xml:lang="de">hat Namen eines Geografikums</rdfs:label>
  <skos:definition xml:lang="de">Setzt ein Geografikum mit einem Wort, einem Zeichen oder einer Gruppe von Wörtern und/oder Zeichen, unter dem/der ein Geografikum bekannt ist, in Beziehung.</skos:definition>
  <rdakit:toolkitLabel xml:lang="de">Name eines Geografikums</rdakit:toolkitLabel>
  <rdakit:toolkitDefinition xml:lang="de">Ein Wort, ein Zeichen oder eine Gruppe von Wörtern und/oder Zeichen, unter dem/der ein Geografikum bekannt ist.</rdakit:toolkitDefinition>
  <rdfs:label xml:lang="ca">té com a nom de lloc</rdfs:label>
  <skos:definition xml:lang="ca">Relaciona un lloc amb una paraula, caràcter i/o grup de paraules o de caràcters pel qual es coneix un lloc.</skos:definition>
  <rdakit:toolkitLabel xml:lang="ca">nom de lloc</rdakit:toolkitLabel>
  <rdakit:toolkitDefinition xml:lang="ca">Paraula, caràcter o grup de paraules o de caràcters pel qual es coneix un lloc.</rdakit:toolkitDefinition>
  <reg:name xml:lang="fi">paikannimi</reg:name>
  <rdfs:label xml:lang="fi">paikannimi</rdfs:label>
  <reg:lexicalAlias rdf:resource="http://rdaregistry.info/Elements/p/paikannimi.fi" />
  <skos:definition xml:lang="fi">Liittää paikan sanaan, merkkiin tai joukkoon sanoihin ja/tai merkkejä, joilla paikka tunnetaan.</skos:definition>
  <rdakit:toolkitLabel xml:lang="fi">paikannimi</rdakit:toolkitLabel>
  <rdakit:toolkitDefinition xml:lang="fi">Sana, merkki tai joukko sanoja ja/tai merkkejä, joilla paikka tunnetaan.</rdakit:toolkitDefinition>
  <reg:name xml:lang="fr">nomDeLieu</reg:name>
  <rdfs:label xml:lang="fr">a pour nom de lieu</rdfs:label>
  <reg:lexicalAlias rdf:resource="http://rdaregistry.info/Elements/p/nomDeLieu.fr" />
  <skos:definition xml:lang="fr">Met un lieu en relation avec un mot, un caractère ou un groupe de mots ou de caractères sous lequel un lieu est connu.</skos:definition>
  <rdakit:toolkitLabel xml:lang="fr">nom de lieu</rdakit:toolkitLabel>
  <rdakit:toolkitDefinition xml:lang="fr">Mot, caractère ou groupe de mots ou de caractères sous lequel un lieu est connu.</rdakit:toolkitDefinition>
  <rdakit:toolkitLabel xml:lang="no">stedsnavn</rdakit:toolkitLabel>
  <rdakit:toolkitDefinition xml:lang="no">Et ord, et tegn eller en gruppe av ord eller tegn som et sted er kjent under.</rdakit:toolkitDefinition>
  <reg:name xml:lang="el">όνομαΤουΤόπου</reg:name>
  <rdfs:label xml:lang="el">έχει όνομα του τόπου</rdfs:label>
  <reg:lexicalAlias rdf:resource="http://rdaregistry.info/Elements/p/όνομαΤουΤόπου.el" />
  <skos:definition xml:lang="el">Συνδέει έναν τόπο με μια λέξη, έναν χαρακτήρα ή μια ομάδα λέξεων ή/και χαρακτήρων με τους οποίους είναι γνωστός ένας τόπος.</skos:definition>
  <rdakit:toolkitLabel xml:lang="el">όνομα του τόπου</rdakit:toolkitLabel>
  <rdakit:toolkitDefinition xml:lang="el">Μια λέξη, ένας χαρακτήρας ή μια ομάδα λέξεων ή χαρακτήρων με τους οποίους είναι γνωστός ένας τόπος.</rdakit:toolkitDefinition>
  <rdfs:subPropertyOf rdf:resource="http://rdaregistry.info/Elements/p/P70019" />
  <reg:hasSubproperty rdf:resource="http://rdaregistry.info/Elements/p/object/P70001" />
  <rdakit:hasElementType xml:lang="">3</rdakit:hasElementType>
  <reg:name xml:lang="hu">Helyneve</reg:name>
  <rdfs:label xml:lang="hu">van helyneve</rdfs:label>
  <skos:definition xml:lang="hu">Egy helyet hozzákapcsol egy szóhoz, karakterhez, vagy szavak és/vagy karakterek egy csoportjához, amely által egy helyet ismernek.</skos:definition>
  <rdakit:toolkitLabel xml:lang="hu">helynév</rdakit:toolkitLabel>
  <rdakit:toolkitDefinition xml:lang="hu">Egy szó, karakter, vagy szavak vagy karakterek egy csoportja, amely által egy helyet ismernek.</rdakit:toolkitDefinition>
  <reg:hasSubproperty rdf:resource="http://rdaregistry.info/Elements/p/P70002" />
  <reg:hasSubproperty rdf:resource="http://rdaregistry.info/Elements/p/P70003" />
  <rdfs:subPropertyOf rdf:resource="http://rdaregistry.info/Elements/x/P00019" />
</rdf:Description>

<!-- Property: has variant name of place -->
<rdf:Description rdf:about="http://rdaregistry.info/Elements/p/P70003">
  <rdfs:isDefinedBy rdf:resource="http://rdaregistry.info/Elements/p/" />
  <reg:status rdf:resource="http://metadataregistry.org/uri/RegStatus/1001" />
  <rdfs:label xml:lang="en">has variant name of place</rdfs:label>
  <rdf:type rdf:resource="http://www.w3.org/1999/02/22-rdf-syntax-ns#Property" />
  <reg:name xml:lang="en">variantNameOfPlace</reg:name>
  <skos:definition xml:lang="en">Relates a place to a name of place that is not selected for preference in a specific application or context.</skos:definition>
  <rdfs:subPropertyOf rdf:resource="http://rdaregistry.info/Elements/p/P70001" />
  <rdfs:domain rdf:resource="http://rdaregistry.info/Elements/c/C10009" />
  <reg:lexicalAlias rdf:resource="http://rdaregistry.info/Elements/p/variantNameOfPlace.en" />
  <rdakit:toolkitLabel xml:lang="en">variant name of place</rdakit:toolkitLabel>
  <rdakit:toolkitDefinition xml:lang="en">A name of place that is not selected for preference in a specific application or context.</rdakit:toolkitDefinition>
  <reg:hasUnconstrained rdf:resource="http://rdaregistry.info/Elements/u/P60880" />
  <rdakit:instructionNumber xml:lang="">16.2.3</rdakit:instructionNumber>
  <reg:hasSubproperty rdf:resource="http://rdaregistry.info/Elements/p/datatype/P70003" />
  <skos:scopeNote xml:lang="en">Variant name for place includes a name found in reference sources, or a name resulting from a different transliteration of a name, etc.</skos:scopeNote>
  <reg:name xml:lang="da">variantnavnForEtSted</reg:name>
  <rdfs:label xml:lang="da">har variantnavn for et sted</rdfs:label>
  <reg:lexicalAlias rdf:resource="http://rdaregistry.info/Elements/p/variantnavnForEtSted.da" />
  <skos:definition xml:lang="da">Relaterer et sted til en navn eller navneform, hvorunder et sted er kendt, og som adskiller sig fra det navn eller den navneform, der er valgt som foretrukket navn.</skos:definition>
  <rdakit:toolkitLabel xml:lang="da">variantnavn for et sted</rdakit:toolkitLabel>
  <rdakit:toolkitDefinition xml:lang="da">Navn eller navneform, hvorunder et sted er kendt, og som adskiller sig fra det navn eller den navneform, der er valgt som foretrukket navn.</rdakit:toolkitDefinition>
  <reg:name xml:lang="vi">tênKhácCủaĐịaĐiểm</reg:name>
  <rdfs:label xml:lang="vi">có tên khác của địa điểm</rdfs:label>
  <skos:definition xml:lang="vi">Liên kết địa điểm với tên hoặc hình thái của tên mà theo đó địa điểm được biết đến khác với tên hoặc hình thái của tên được chọn lựa như là tên ưu tiên.</skos:definition>
  <skos:scopeNote xml:lang="vi">Tên khác của địa điểm bao gồm tên hoặc hình thái của tên được tìm thấy trong các nguồn tham khảo, hoặc tên sinh ra từ phiên âm khác nhau của tên, v.v...</skos:scopeNote>
  <rdakit:toolkitLabel xml:lang="vi">tên khác của địa điểm</rdakit:toolkitLabel>
  <rdakit:toolkitDefinition xml:lang="vi">Tên hoặc hình thái của tên mà theo đó địa điểm được biết đến khác với tên hoặc hình thái của tên được chọn lựa như là tên ưu tiên.</rdakit:toolkitDefinition>
  <rdfs:label xml:lang="de">hat abweichenden Name eines Geografikums</rdfs:label>
  <skos:definition xml:lang="de">Setzt einen Namen oder eine Namensform, unter dem/der ein Geografikum bekannt ist, der/die sich von dem Namen oder der Namensform unterscheidet, der/die als bevorzugter Name gewählt wurde, in Beziehung.</skos:definition>
  <skos:scopeNote xml:lang="de">Zu einem abweichenden Namen eines Geografikums gehört ein Name oder eine Namensform wie er/sie in Nachschlagewerken gefunden wird/werden, ein Titel der sich aus einer abweichenden Transliteration ergibt usw.</skos:scopeNote>
  <rdakit:toolkitLabel xml:lang="de">Abweichender Name eines Geografikums</rdakit:toolkitLabel>
  <rdakit:toolkitDefinition xml:lang="de">Ein Name oder eine Namensform, unter dem/der ein Geografikum bekannt ist, der/die sich von dem Namen oder der Namensform unterscheidet, der/die als bevorzugter Name gewählt wurde.</rdakit:toolkitDefinition>
  <rdfs:label xml:lang="ca">té com a variant de nom de lloc</rdfs:label>
  <skos:definition xml:lang="ca">Relaciona un lloc amb un nom o forma de nom pel qual es coneix un lloc i que difereix del nom o la forma de nom triat com a nom preferit.</skos:definition>
  <skos:scopeNote xml:lang="ca">La variant de nom de lloc inclou un nom o forma de nom trobat en les fonts de referència, o un nom que és el resultat d’una transliteració diferent d’un nom, etc.</skos:scopeNote>
  <rdakit:toolkitLabel xml:lang="ca">variant de nom de lloc</rdakit:toolkitLabel>
  <rdakit:toolkitDefinition xml:lang="ca">Nom o forma de nom pel qual es coneix un lloc i que difereix del nom o la forma de nom triat com a nom preferit.</rdakit:toolkitDefinition>
  <reg:name xml:lang="fi">paikanVarianttinimi</reg:name>
  <rdfs:label xml:lang="fi">paikan varianttinimi</rdfs:label>
  <reg:lexicalAlias rdf:resource="http://rdaregistry.info/Elements/p/paikanVarianttinimi.fi" />
  <skos:definition xml:lang="fi">Liittää paikan ensisijaisesta nimestä tai nimenmuodosta poikkeavaan nimeen tai nimenmuotoon, jolla paikka tunnetaan.</skos:definition>
  <skos:scopeNote xml:lang="fi">Paikan varianttinimi on nimi tai nimenmuoto, jota on käytetty tietolähteissä tai joka on translitteroitu eri tavoin tms.</skos:scopeNote>
  <rdakit:toolkitLabel xml:lang="fi">paikan varianttinimi</rdakit:toolkitLabel>
  <rdakit:toolkitDefinition xml:lang="fi">Ensisijaisesta nimestä tai nimenmuodosta poikkeava nimi tai nimenmuoto, jolla paikka tunnetaan.</rdakit:toolkitDefinition>
  <reg:name xml:lang="fr">varianteDeNomDeLieu</reg:name>
  <rdfs:label xml:lang="fr">a pour variante de nom de lieu</rdfs:label>
  <reg:lexicalAlias rdf:resource="http://rdaregistry.info/Elements/p/varianteDeNomDeLieu.fr" />
  <skos:definition xml:lang="fr">Met un lieu en relation avec un nom ou une forme de nom sous laquelle un lieu est connu et qui diffère d’un nom ou d’une forme de nom choisie comme nom privilégié.</skos:definition>
  <skos:scopeNote xml:lang="fr">Une variante de nom de lieu comprend un nom ou une forme de nom trouvée dans les sources de référence ou un nom qui résulte d’une translittération différente d’un nom, etc.</skos:scopeNote>
  <rdakit:toolkitLabel xml:lang="fr">variante de nom de lieu</rdakit:toolkitLabel>
  <rdakit:toolkitDefinition xml:lang="fr">Nom ou forme de nom sous laquelle un lieu est connu et qui diffère du nom ou de la forme de nom choisie comme nom privilégié.</rdakit:toolkitDefinition>
  <rdakit:toolkitLabel xml:lang="no">variantform av stedsnavn</rdakit:toolkitLabel>
  <rdakit:toolkitDefinition xml:lang="no">Et navn eller en navneform som et sted er kjent under og som avviker fra navnet eller navneformen som er valgt som det foretrukne navnet.</rdakit:toolkitDefinition>
  <reg:name xml:lang="el">εναλλακτικόΌνομαΓιαΤόπο</reg:name>
  <rdfs:label xml:lang="el">έχει εναλλακτικό όνομα για τόπο</rdfs:label>
  <reg:lexicalAlias rdf:resource="http://rdaregistry.info/Elements/p/εναλλακτικόΌνομαΓιαΤόπο.el" />
  <skos:definition xml:lang="el">Συνδέει έναν τόπο με ένα όνομα ή μια μορφή του ονόματος με το οποίο είναι γνωστός ένας τόπος, το οποίο διαφέρει από ένα όνομα ή μια μορφή ονόματος που επιλέγεται ως το προτιμώμενο όνομα.</skos:definition>
  <skos:scopeNote xml:lang="el">Το εναλλακτικό όνομα για έναν τόπο περιλαμβάνει ένα όνομα ή μια μορφή του ονόματος που εντοπίζεται στις πηγές αναφοράς ή ένα όνομα που προκύπτει από έναν διαφορετικό μεταγραμματισμό ενός ονόματος κ.λπ.</skos:scopeNote>
  <rdakit:toolkitLabel xml:lang="el">εναλλακτικό όνομα για τόπο</rdakit:toolkitLabel>
  <rdakit:toolkitDefinition xml:lang="el">Ένα όνομα ή μια μορφή του ονόματος με το οποίο είναι γνωστός ένας τόπος, το οποίο διαφέρει από ένα όνομα ή μια μορφή ονόματος που επιλέγεται ως το προτιμώμενο όνομα.</rdakit:toolkitDefinition>
  <reg:hasSubproperty rdf:resource="http://rdaregistry.info/Elements/p/object/P70003" />
  <rdakit:hasElementType xml:lang="">3</rdakit:hasElementType>
  <reg:name xml:lang="hu">HelyNévváltozata</reg:name>
  <rdfs:label xml:lang="hu">van helynévváltozata</rdfs:label>
  <skos:definition xml:lang="hu">Egy helyet hozzákapcsol egy névhez vagy névformához, amely által egy helyet ismernek, amely különbözik attól a névtől vagy névformától, amelyet preferált névnek választottak.</skos:definition>
  <skos:scopeNote xml:lang="hu">A helynévváltozat magában foglal egy nevet vagy névformát, amely a referenszforrásokban található, vagy egy nevet, amely egy név stb. eltérő átírásából származik.</skos:scopeNote>
  <rdakit:toolkitLabel xml:lang="hu">helynévváltozat</rdakit:toolkitLabel>
  <rdakit:toolkitDefinition xml:lang="hu">Egy név vagy névforma, amely által egy helyet ismernek, amely különbözik attól a névtől vagy névformától, amelyet preferált névként választottak.</rdakit:toolkitDefinition>
  <rdfs:subPropertyOf rdf:resource="http://rdaregistry.info/Elements/x/P00023" />
  <skos:altLabel xml:lang="en">variant name for place</skos:altLabel>
</rdf:Description>

<!-- Property: has preferred name of place -->
<rdf:Description rdf:about="http://rdaregistry.info/Elements/p/P70002">
  <rdfs:isDefinedBy rdf:resource="http://rdaregistry.info/Elements/p/" />
  <reg:status rdf:resource="http://metadataregistry.org/uri/RegStatus/1001" />
  <rdfs:label xml:lang="en">has preferred name of place</rdfs:label>
  <rdf:type rdf:resource="http://www.w3.org/1999/02/22-rdf-syntax-ns#Property" />
  <reg:name xml:lang="en">preferredNameOfPlace</reg:name>
  <skos:definition xml:lang="en">Relates a place to a name of place that is selected for preference in a specific application or context.</skos:definition>
  <rdfs:subPropertyOf rdf:resource="http://rdaregistry.info/Elements/p/P70001" />
  <rdfs:domain rdf:resource="http://rdaregistry.info/Elements/c/C10009" />
  <reg:lexicalAlias rdf:resource="http://rdaregistry.info/Elements/p/preferredNameOfPlace.en" />
  <rdakit:toolkitLabel xml:lang="en">preferred name of place</rdakit:toolkitLabel>
  <rdakit:toolkitDefinition xml:lang="en">A name of place that is selected for preference in a specific application or context.</rdakit:toolkitDefinition>
  <reg:hasUnconstrained rdf:resource="http://rdaregistry.info/Elements/u/P60548" />
  <rdakit:instructionNumber xml:lang="">16.2.2</rdakit:instructionNumber>
  <reg:hasSubproperty rdf:resource="http://rdaregistry.info/Elements/p/datatype/P70002" />
  <reg:name xml:lang="da">foretrukkenNavneformForEtSted</reg:name>
  <rdfs:label xml:lang="da">har foretrukken navneform for et sted</rdfs:label>
  <reg:lexicalAlias rdf:resource="http://rdaregistry.info/Elements/p/foretrukkenNavneformForEtSted.da" />
  <skos:definition xml:lang="da">Relaterer et sted til et navn eller en navneform, der er valgt til identifikation af et sted.</skos:definition>
  <rdakit:toolkitLabel xml:lang="da">foretrukken navneform for et sted</rdakit:toolkitLabel>
  <rdakit:toolkitDefinition xml:lang="da">Navn eller navneform, der er valgt til identifikation af et sted.</rdakit:toolkitDefinition>
  <reg:name xml:lang="vi">tênƯuTiênCủaĐịaĐiểm</reg:name>
  <rdfs:label xml:lang="vi">có tên ưu tiên của địa điểm</rdfs:label>
  <skos:definition xml:lang="vi">Liên kết địa điểm với tên hoặc hình thái của tên được chọn lựa để nhận dạng địa điểm.</skos:definition>
  <rdakit:toolkitLabel xml:lang="vi">tên ưu tiên của địa điểm</rdakit:toolkitLabel>
  <rdakit:toolkitDefinition xml:lang="vi">Tên hoặc hình thái của tên được chọn lựa để nhận dạng địa điểm.</rdakit:toolkitDefinition>
  <rdfs:label xml:lang="de">hat Bevorzugter Name eines Geografikums</rdfs:label>
  <skos:definition xml:lang="de">Setzt einen Namen oder eine Namensform, der/die gewählt wird, um ein Geografikum zu identifizieren, in Beziehung.</skos:definition>
  <rdakit:toolkitLabel xml:lang="de">Bevorzugter Name eines Geografikums</rdakit:toolkitLabel>
  <rdakit:toolkitDefinition xml:lang="de">Ein Name oder eine Namensform, der/die gewählt wird, um ein Geografikum zu identifizieren.</rdakit:toolkitDefinition>
  <rdfs:label xml:lang="ca">té com a nom preferit de lloc</rdfs:label>
  <skos:definition xml:lang="ca">Relaciona un lloc amb un nom o forma de nom triat per identificar un lloc.</skos:definition>
  <rdakit:toolkitLabel xml:lang="ca">nom preferit de lloc</rdakit:toolkitLabel>
  <rdakit:toolkitDefinition xml:lang="ca">Nom o forma de nom triat per identificar un lloc.</rdakit:toolkitDefinition>
  <reg:name xml:lang="fi">paikanEnsisijainenNimi</reg:name>
  <rdfs:label xml:lang="fi">paikan ensisijainen nimi</rdfs:label>
  <reg:lexicalAlias rdf:resource="http://rdaregistry.info/Elements/p/paikanEnsisijainenNimi.fi" />
  <skos:definition xml:lang="fi">Liittää paikan nimeen tai nimenmuotoon, joka on valittu identifioimaan paikkaa.</skos:definition>
  <rdakit:toolkitLabel xml:lang="fi">paikan ensisijainen nimi</rdakit:toolkitLabel>
  <rdakit:toolkitDefinition xml:lang="fi">Nimi tai nimenmuoto, joka on valittu identifioimaan paikkaa.</rdakit:toolkitDefinition>
  <reg:name xml:lang="fr">nomPrivilégiéDunLieu</reg:name>
  <rdfs:label xml:lang="fr">a pour nom privilégié d’un lieu</rdfs:label>
  <reg:lexicalAlias rdf:resource="http://rdaregistry.info/Elements/p/nomPrivilégiéDunLieu.fr" />
  <skos:definition xml:lang="fr">Met un lieu en relation avec un nom ou une forme de nom choisie pour identifier un lieu.</skos:definition>
  <rdakit:toolkitLabel xml:lang="fr">nom privilégié d’un lieu</rdakit:toolkitLabel>
  <rdakit:toolkitDefinition xml:lang="fr">Nom ou forme de nom choisie pour identifier un lieu.</rdakit:toolkitDefinition>
  <rdakit:toolkitLabel xml:lang="no">foretrukket stedsnavn</rdakit:toolkitLabel>
  <rdakit:toolkitDefinition xml:lang="no">Et navn eller en navneform som er valgt for å identifisere et sted.</rdakit:toolkitDefinition>
  <reg:name xml:lang="el">προτιμώμενοΌνομαΓιαΤόπο</reg:name>
  <rdfs:label xml:lang="el">έχει προτιμώμενο όνομα για τόπο</rdfs:label>
  <reg:lexicalAlias rdf:resource="http://rdaregistry.info/Elements/p/προτιμώμενοΌνομαΓιαΤόπο.el" />
  <skos:definition xml:lang="el">Συνδέει έναν τόπο με ένα όνομα ή μια μορφή του ονόματος που επιλέγεται για την ταύτιση ενός τόπου.</skos:definition>
  <rdakit:toolkitLabel xml:lang="el">προτιμώμενο όνομα για τόπο</rdakit:toolkitLabel>
  <rdakit:toolkitDefinition xml:lang="el">Ένα όνομα ή μια μορφή του ονόματος που επιλέγεται για την ταύτιση ενός τόπου.</rdakit:toolkitDefinition>
  <reg:hasSubproperty rdf:resource="http://rdaregistry.info/Elements/p/object/P70002" />
  <rdakit:hasElementType xml:lang="">3</rdakit:hasElementType>
  <reg:name xml:lang="hu">HelypreferáltNeve</reg:name>
  <rdfs:label xml:lang="hu">van preferált helyneve</rdfs:label>
  <skos:definition xml:lang="hu">Egy helyet hozzákapcsol egy névhez vagy névformához, amelyet egy hely azonosítására és megnevezésére választottak.</skos:definition>
  <rdakit:toolkitLabel xml:lang="hu">preferált helynév</rdakit:toolkitLabel>
  <rdakit:toolkitDefinition xml:lang="hu">Egy név vagy névforma, amelyet egy hely azonosítására választottak.</rdakit:toolkitDefinition>
  <rdfs:subPropertyOf rdf:resource="http://rdaregistry.info/Elements/x/P00021" />
  <skos:altLabel xml:lang="en">preferred name for place</skos:altLabel>
</rdf:Description>

<!-- Property: is subject place of -->
<rdf:Description rdf:about="http://rdaregistry.info/Elements/p/P70017">
  <rdfs:isDefinedBy rdf:resource="http://rdaregistry.info/Elements/p/" />
  <reg:status rdf:resource="http://metadataregistry.org/uri/RegStatus/1001" />
  <rdf:type rdf:resource="http://www.w3.org/1999/02/22-rdf-syntax-ns#Property" />
  <rdfs:label xml:lang="en">is subject place of</rdfs:label>
  <reg:lexicalAlias rdf:resource="http://rdaregistry.info/Elements/p/subjecfPlaceOf.en" />
  <skos:definition xml:lang="en">Relates a place to a work that is about a place.</skos:definition>
  <rdfs:domain rdf:resource="http://rdaregistry.info/Elements/c/C10009" />
  <reg:hasSubproperty rdf:resource="http://rdaregistry.info/Elements/p/datatype/P70017" />
  <reg:hasSubproperty rdf:resource="http://rdaregistry.info/Elements/p/object/P70017" />
  <rdfs:subPropertyOf rdf:resource="http://rdaregistry.info/Elements/p/P70004" />
  <reg:name xml:lang="en">subjecfPlaceOf</reg:name>
  <reg:name xml:lang="da">emneForSted</reg:name>
  <rdfs:label xml:lang="da">er emne for sted</rdfs:label>
  <reg:lexicalAlias rdf:resource="http://rdaregistry.info/Elements/p/emneForSted.da" />
  <skos:definition xml:lang="da">Relaterer et sted til et verk der handler om et sted.</skos:definition>
  <reg:name xml:lang="vi">chủĐềCủaĐịaĐiểm</reg:name>
  <rdfs:label xml:lang="vi">là chủ đề của (địa điểm)</rdfs:label>
  <skos:definition xml:lang="vi">Liên kết địa điểm với tác phẩm về địa điểm.</skos:definition>
  <rdfs:label xml:lang="ca">és matèria de (lloc)</rdfs:label>
  <skos:definition xml:lang="ca">Relaciona un lloc amb una obra que tracta d’un lloc.</skos:definition>
  <reg:name xml:lang="fi">paikkaAiheenaTeoksessa</reg:name>
  <rdfs:label xml:lang="fi">paikka aiheena teoksessa</rdfs:label>
  <reg:lexicalAlias rdf:resource="http://rdaregistry.info/Elements/p/paikkaAiheenaTeoksessa.fi" />
  <skos:definition xml:lang="fi">Liittää paikan teokseen, jonka aiheena paikka on.</skos:definition>
  <reg:name xml:lang="fr">sujetDeLieu</reg:name>
  <rdfs:label xml:lang="fr">est un sujet de (lieu)</rdfs:label>
  <reg:lexicalAlias rdf:resource="http://rdaregistry.info/Elements/p/sujetDeLieu.fr" />
  <skos:definition xml:lang="fr">Met un lieu en relation avec une œuvre qui traite d’un lieu.</skos:definition>
  <reg:name xml:lang="el">θέμαΤουΤόπου</reg:name>
  <rdfs:label xml:lang="el">είναι θέμα του (τόπος)</rdfs:label>
  <reg:lexicalAlias rdf:resource="http://rdaregistry.info/Elements/p/θέμαΤουΤόπου.el" />
  <skos:definition xml:lang="el">Συνδέει έναν τόπο με ένα έργο που αναφέρεται σε έναν τόπο.</skos:definition>
  <rdakit:toolkitLabel xml:lang="en">subject place of</rdakit:toolkitLabel>
  <rdakit:toolkitDefinition xml:lang="en">A work that is about a place.</rdakit:toolkitDefinition>
  <rdakit:hasElementType xml:lang="">2</rdakit:hasElementType>
  <skos:altLabel xml:lang="en">subject of (place)</skos:altLabel>
  <reg:name xml:lang="hu">Helytárgya</reg:name>
  <rdfs:label xml:lang="hu">tárgya (hely)</rdfs:label>
  <skos:definition xml:lang="hu">Egy helyet hozzákapcsol egy műhöz, amely egy helyről szól.</skos:definition>
  <rdfs:subPropertyOf rdf:resource="http://rdaregistry.info/Elements/x/P00014" />
  <reg:hasSubproperty rdf:resource="http://rdaregistry.info/Elements/p/P70054" />
  <reg:hasUnconstrained rdf:resource="http://rdaregistry.info/Elements/u/P60806" />
</rdf:Description>

<!-- Property: has identifier for place -->
<rdf:Description rdf:about="http://rdaregistry.info/Elements/p/P70020">
  <rdfs:isDefinedBy rdf:resource="http://rdaregistry.info/Elements/p/" />
  <reg:status rdf:resource="http://metadataregistry.org/uri/RegStatus/1001" />
  <rdf:type rdf:resource="http://www.w3.org/1999/02/22-rdf-syntax-ns#Property" />
  <reg:name xml:lang="en">identifierForPlace</reg:name>
  <rdfs:label xml:lang="en">has identifier for place</rdfs:label>
  <reg:lexicalAlias rdf:resource="http://rdaregistry.info/Elements/p/identifierForPlace.en" />
  <skos:definition xml:lang="en">Relates a place to an appellation of place that consists of a code, number, or other string, usually independent of natural language and social naming conventions, used to identify a place.</skos:definition>
  <rdfs:domain rdf:resource="http://rdaregistry.info/Elements/c/C10009" />
  <rdakit:toolkitLabel xml:lang="en">identifier for place</rdakit:toolkitLabel>
  <rdakit:toolkitDefinition xml:lang="en">An appellation of place that consists of a code, number, or other string, usually independent of natural language and social naming conventions, used to identify a place.</rdakit:toolkitDefinition>
  <reg:hasUnconstrained rdf:resource="http://rdaregistry.info/Elements/u/P60919" />
  <reg:hasSubproperty rdf:resource="http://rdaregistry.info/Elements/p/object/P70020" />
  <rdfs:subPropertyOf rdf:resource="http://rdaregistry.info/Elements/p/P70019" />
  <rdakit:hasElementType xml:lang="">3</rdakit:hasElementType>
  <reg:hasSubproperty rdf:resource="http://rdaregistry.info/Elements/p/datatype/P70020" />
  <rdakit:instructionNumber xml:lang="">16.3</rdakit:instructionNumber>
  <rdfs:subPropertyOf rdf:resource="http://rdaregistry.info/Elements/x/P00018" />
</rdf:Description>

<!-- Property: is jurisdiction governed of -->
<rdf:Description rdf:about="http://rdaregistry.info/Elements/p/P70051">
  <rdfs:isDefinedBy rdf:resource="http://rdaregistry.info/Elements/p/" />
  <reg:status rdf:resource="http://metadataregistry.org/uri/RegStatus/1001" />
  <rdfs:label xml:lang="en">is jurisdiction governed of</rdfs:label>
  <rdf:type rdf:resource="http://www.w3.org/1999/02/22-rdf-syntax-ns#Property" />
  <reg:name xml:lang="en">jurisdictionGovernedOf</reg:name>
  <reg:lexicalAlias rdf:resource="http://rdaregistry.info/Elements/p/jurisdictionGovernedOf.en" />
  <skos:definition xml:lang="en">Relates a place that is a jurisdiction to a corporate body that is a government of a jurisdiction governed by a law, regulation, etc., that was enacted by another government.</skos:definition>
  <rdfs:domain rdf:resource="http://rdaregistry.info/Elements/c/C10009" />
  <rdakit:hasElementType xml:lang="">2</rdakit:hasElementType>
  <rdfs:subPropertyOf rdf:resource="http://rdaregistry.info/Elements/p/P70016" />
  <reg:hasUnconstrained rdf:resource="http://rdaregistry.info/Elements/u/P60015" />
  <rdakit:toolkitLabel xml:lang="en">jurisdiction governed of</rdakit:toolkitLabel>
  <rdakit:toolkitDefinition xml:lang="en">A corporate body that is a government of a jurisdiction governed by a law, regulation, etc., that was enacted by another government.</rdakit:toolkitDefinition>
  <reg:hasSubproperty rdf:resource="http://rdaregistry.info/Elements/p/datatype/P70051" />
</rdf:Description>

<!-- Property: has related agent of place -->
<rdf:Description rdf:about="http://rdaregistry.info/Elements/p/P70008">
  <rdfs:isDefinedBy rdf:resource="http://rdaregistry.info/Elements/p/" />
  <reg:status rdf:resource="http://metadataregistry.org/uri/RegStatus/1001" />
  <rdf:type rdf:resource="http://www.w3.org/1999/02/22-rdf-syntax-ns#Property" />
  <reg:name xml:lang="en">relatedAgentOfPlace</reg:name>
  <rdfs:label xml:lang="en">has related agent of place</rdfs:label>
  <reg:lexicalAlias rdf:resource="http://rdaregistry.info/Elements/p/relatedAgentOfPlace.en" />
  <skos:definition xml:lang="en">Relates a place to an agent who is associated with a place.</skos:definition>
  <rdfs:domain rdf:resource="http://rdaregistry.info/Elements/c/C10009" />
  <reg:hasSubproperty rdf:resource="http://rdaregistry.info/Elements/p/datatype/P70008" />
  <rdfs:subPropertyOf rdf:resource="http://rdaregistry.info/Elements/p/P70013" />
  <reg:hasSubproperty rdf:resource="http://rdaregistry.info/Elements/p/P70009" />
  <reg:hasSubproperty rdf:resource="http://rdaregistry.info/Elements/p/P70014" />
  <reg:name xml:lang="da">relateretAgentSted</reg:name>
  <rdfs:label xml:lang="da">har relateret agent (sted)</rdfs:label>
  <reg:lexicalAlias rdf:resource="http://rdaregistry.info/Elements/p/relateretAgentSted.da" />
  <skos:definition xml:lang="da">Relaterer et sted til en agent der er knyttet til et beskrevet sted.</skos:definition>
  <reg:name xml:lang="vi">địaĐiểmTácNhânCóLiênQuan</reg:name>
  <rdfs:label xml:lang="vi">có tác nhân có liên quan (địa điểm)</rdfs:label>
  <skos:definition xml:lang="vi">Liên kết địa điểm với tác nhân liên quan tới địa điểm đang được mô tả.</skos:definition>
  <rdfs:label xml:lang="ca">té com a agent relacionat (lloc)</rdfs:label>
  <skos:definition xml:lang="ca">Relaciona un lloc amb un agent associat amb un lloc que es descriu.</skos:definition>
  <reg:name xml:lang="fi">paikkaanLiittyvaToimija</reg:name>
  <rdfs:label xml:lang="fi">paikkaan liittyvä toimija</rdfs:label>
  <reg:lexicalAlias rdf:resource="http://rdaregistry.info/Elements/p/paikkaanLiittyvaToimija.fi" />
  <skos:definition xml:lang="fi">Liittää paikan toimijaan, johon kuvailun kohteena oleva paikka liittyy.</skos:definition>
  <reg:name xml:lang="fr">agentEnRelationLieu</reg:name>
  <rdfs:label xml:lang="fr">a pour agent en relation (lieu)</rdfs:label>
  <reg:lexicalAlias rdf:resource="http://rdaregistry.info/Elements/p/agentEnRelationLieu.fr" />
  <skos:definition xml:lang="fr">Met un lieu en relation avec un agent associé à un lieu décrit.</skos:definition>
  <reg:name xml:lang="el">σχετικόςΦορέαςΤόπος</reg:name>
  <rdfs:label xml:lang="el">έχει σχετικό φορέα (τόπος)</rdfs:label>
  <reg:lexicalAlias rdf:resource="http://rdaregistry.info/Elements/p/σχετικόςΦορέαςΤόπος.el" />
  <skos:definition xml:lang="el">Συνδέει έναν τόπο με έναν φορέα που συνδέεται με έναν περιγραφόμενο τόπο.</skos:definition>
  <rdakit:toolkitLabel xml:lang="en">related agent of place</rdakit:toolkitLabel>
  <rdakit:toolkitDefinition xml:lang="en">An agent who is associated with a place.</rdakit:toolkitDefinition>
  <rdakit:hasElementType xml:lang="">1</rdakit:hasElementType>
  <rdfs:subPropertyOf rdf:resource="http://rdaregistry.info/Elements/x/P00006" />
  <reg:name xml:lang="hu">kapcsolódóÁgensHely</reg:name>
  <rdfs:label xml:lang="hu">van kapcsolódó ágense (hely)</rdfs:label>
  <skos:definition xml:lang="hu">Egy helyet hozzákapcsol egy ágenshez (személyhez, családhoz vagy testülethez), aki/amely kötődik egy éppen leírt helyhez.</skos:definition>
  <reg:hasUnconstrained rdf:resource="http://rdaregistry.info/Elements/u/P61011" />
</rdf:Description>

<!-- Property: has related family of place -->
<rdf:Description rdf:about="http://rdaregistry.info/Elements/p/P70015">
  <rdfs:isDefinedBy rdf:resource="http://rdaregistry.info/Elements/p/" />
  <reg:status rdf:resource="http://metadataregistry.org/uri/RegStatus/1001" />
  <rdfs:subPropertyOf rdf:resource="http://rdaregistry.info/Elements/p/P70009" />
  <rdf:type rdf:resource="http://www.w3.org/1999/02/22-rdf-syntax-ns#Property" />
  <reg:name xml:lang="en">relatedFamilyOfPlace</reg:name>
  <rdfs:label xml:lang="en">has related family of place</rdfs:label>
  <reg:lexicalAlias rdf:resource="http://rdaregistry.info/Elements/p/relatedFamilyOfPlace.en" />
  <skos:definition xml:lang="en">Relates a place to a family who is associated with a place.</skos:definition>
  <rdfs:domain rdf:resource="http://rdaregistry.info/Elements/c/C10009" />
  <reg:hasSubproperty rdf:resource="http://rdaregistry.info/Elements/p/P70015" />
  <reg:hasSubproperty rdf:resource="http://rdaregistry.info/Elements/p/datatype/P70015" />
  <reg:name xml:lang="da">relateretFamilieSted</reg:name>
  <rdfs:label xml:lang="da">har relateret familie (sted)</rdfs:label>
  <reg:lexicalAlias rdf:resource="http://rdaregistry.info/Elements/p/relateretFamilieSted.da" />
  <skos:definition xml:lang="da">Relaterer et sted til en familie der er knyttet til et beskrevet sted.</skos:definition>
  <reg:name xml:lang="vi">địaĐiểmGiaĐìnhCóLiênQuan</reg:name>
  <rdfs:label xml:lang="vi">có gia đình có liên quan (địa điểm)</rdfs:label>
  <skos:definition xml:lang="vi">Liên kết địa điểm với gia đình liên quan tới địa điểm đang được mô tả.</skos:definition>
  <rdfs:label xml:lang="ca">té com a família relacionada (lloc)</rdfs:label>
  <skos:definition xml:lang="ca">Relaciona un lloc amb una família associada amb un lloc que es descriu.</skos:definition>
  <reg:name xml:lang="fi">paikkaanLiittyvaSuku</reg:name>
  <rdfs:label xml:lang="fi">paikkaan liittyvä suku</rdfs:label>
  <reg:lexicalAlias rdf:resource="http://rdaregistry.info/Elements/p/paikkaanLiittyvaSuku.fi" />
  <skos:definition xml:lang="fi">Liittää paikan sukuun, johon kuvailun kohteena oleva paikka liittyy.</skos:definition>
  <reg:name xml:lang="fr">familleEnRelationLieu</reg:name>
  <rdfs:label xml:lang="fr">a pour famille en relation (lieu)</rdfs:label>
  <reg:lexicalAlias rdf:resource="http://rdaregistry.info/Elements/p/familleEnRelationLieu.fr" />
  <skos:definition xml:lang="fr">Met un lieu en relation avec une famille associée à un lieu décrit.</skos:definition>
  <reg:name xml:lang="el">σχετικήΟικογένειαΤόπος</reg:name>
  <rdfs:label xml:lang="el">έχει σχετική οικογένεια (τόπος)</rdfs:label>
  <reg:lexicalAlias rdf:resource="http://rdaregistry.info/Elements/p/σχετικήΟικογένειαΤόπος.el" />
  <skos:definition xml:lang="el">Συνδέει έναν τόπο με μια οικογένεια που συνδέεται με έναν περιγραφόμενο τόπο.</skos:definition>
  <rdakit:toolkitLabel xml:lang="en">related family of place</rdakit:toolkitLabel>
  <rdakit:toolkitDefinition xml:lang="en">A family who is associated with a place.</rdakit:toolkitDefinition>
  <rdakit:hasElementType xml:lang="">1</rdakit:hasElementType>
  <rdfs:subPropertyOf rdf:resource="http://rdaregistry.info/Elements/x/P00008" />
  <reg:name xml:lang="hu">kapcsolódóCsaládHely</reg:name>
  <rdfs:label xml:lang="hu">van kapcsolódó családja (hely)</rdfs:label>
  <skos:definition xml:lang="hu">Egy helyet hozzákapcsol egy családhoz, amely kötődik egy éppen leírt helyhez.</skos:definition>
  <skos:altLabel xml:lang="en">place associated with family of</skos:altLabel>
  <reg:hasUnconstrained rdf:resource="http://rdaregistry.info/Elements/u/P61011" />
</rdf:Description>

<!-- Property: has related place of place -->
<rdf:Description rdf:about="http://rdaregistry.info/Elements/p/P70010">
  <rdfs:isDefinedBy rdf:resource="http://rdaregistry.info/Elements/p/" />
  <reg:status rdf:resource="http://metadataregistry.org/uri/RegStatus/1001" />
  <rdf:type rdf:resource="http://www.w3.org/1999/02/22-rdf-syntax-ns#Property" />
  <reg:name xml:lang="en">relatedPlaceOfPlace</reg:name>
  <rdfs:label xml:lang="en">has related place of place</rdfs:label>
  <reg:lexicalAlias rdf:resource="http://rdaregistry.info/Elements/p/relatedPlaceOfPlace.en" />
  <skos:definition xml:lang="en">Relates a place to a place that is associated with a place.</skos:definition>
  <rdfs:domain rdf:resource="http://rdaregistry.info/Elements/c/C10009" />
  <reg:hasSubproperty rdf:resource="http://rdaregistry.info/Elements/p/datatype/P70010" />
  <rdfs:subPropertyOf rdf:resource="http://rdaregistry.info/Elements/p/P70013" />
  <reg:name xml:lang="da">relateretStedSted</reg:name>
  <rdfs:label xml:lang="da">har relateret sted (sted)</rdfs:label>
  <reg:lexicalAlias rdf:resource="http://rdaregistry.info/Elements/p/relateretStedSted.da" />
  <skos:definition xml:lang="da">Relaterer et sted til et sted der er knyttet til et beskrevet sted.</skos:definition>
  <reg:name xml:lang="vi">địaĐiểmĐịaĐiểmCóLiênQuan</reg:name>
  <rdfs:label xml:lang="vi">có địa điểm có liên quan (địa điểm)</rdfs:label>
  <skos:definition xml:lang="vi">Liên kết địa điểm với địa điểm liên quan tới địa điểm đang được mô tả.</skos:definition>
  <rdfs:label xml:lang="ca">té com a lloc relacionat (lloc)</rdfs:label>
  <skos:definition xml:lang="ca">Relaciona un lloc amb un lloc associat amb un lloc que es descriu.</skos:definition>
  <reg:name xml:lang="fi">paikkaanLiittyvaPaikka</reg:name>
  <rdfs:label xml:lang="fi">paikkaan liittyvä paikka</rdfs:label>
  <reg:lexicalAlias rdf:resource="http://rdaregistry.info/Elements/p/paikkaanLiittyvaPaikka.fi" />
  <skos:definition xml:lang="fi">Liittää paikan paikkaan, johon kuvailun kohteena oleva paikka liittyy.</skos:definition>
  <reg:name xml:lang="fr">lieuEnRelationLieu</reg:name>
  <rdfs:label xml:lang="fr">a pour lieu en relation (lieu)</rdfs:label>
  <reg:lexicalAlias rdf:resource="http://rdaregistry.info/Elements/p/lieuEnRelationLieu.fr" />
  <skos:definition xml:lang="fr">Met un lieu en relation avec un lieu associé à un lieu décrit.</skos:definition>
  <reg:name xml:lang="el">σχετικόςΤόποςΤόπος</reg:name>
  <rdfs:label xml:lang="el">έχει σχετικό τόπο (τόπος)</rdfs:label>
  <reg:lexicalAlias rdf:resource="http://rdaregistry.info/Elements/p/σχετικόςΤόποςΤόπος.el" />
  <skos:definition xml:lang="el">Συνδέει έναν τόπο με έναν τόπο που συνδέεται με έναν περιγραφόμενο τόπο.</skos:definition>
  <rdakit:toolkitLabel xml:lang="en">related place of place</rdakit:toolkitLabel>
  <rdakit:toolkitDefinition xml:lang="en">A place that is associated with a place.</rdakit:toolkitDefinition>
  <rdakit:hasElementType xml:lang="">1</rdakit:hasElementType>
  <rdfs:subPropertyOf rdf:resource="http://rdaregistry.info/Elements/x/P00010" />
  <reg:name xml:lang="hu">kapcsolódóHelyHely</reg:name>
  <rdfs:label xml:lang="hu">van kapcsolódó helye (hely)</rdfs:label>
  <skos:definition xml:lang="hu">Egy helyet hozzákapcsol egy helyhez, amely kötődik egy éppen leírt helyhez.</skos:definition>
  <reg:hasSubproperty rdf:resource="http://rdaregistry.info/Elements/p/P70032" />
  <reg:hasSubproperty rdf:resource="http://rdaregistry.info/Elements/p/P70033" />
  <reg:hasUnconstrained rdf:resource="http://rdaregistry.info/Elements/u/P61016" />
</rdf:Description>

<!-- Property: has related timespan of place -->
<rdf:Description rdf:about="http://rdaregistry.info/Elements/p/P70011">
  <rdfs:isDefinedBy rdf:resource="http://rdaregistry.info/Elements/p/" />
  <reg:status rdf:resource="http://metadataregistry.org/uri/RegStatus/1001" />
  <rdf:type rdf:resource="http://www.w3.org/1999/02/22-rdf-syntax-ns#Property" />
  <reg:name xml:lang="en">relatedTimespanOfPlace</reg:name>
  <rdfs:label xml:lang="en">has related timespan of place</rdfs:label>
  <reg:lexicalAlias rdf:resource="http://rdaregistry.info/Elements/p/relatedTimespanOfPlace.en" />
  <skos:definition xml:lang="en">Relates a place to a timespan that is associated with a place.</skos:definition>
  <rdfs:domain rdf:resource="http://rdaregistry.info/Elements/c/C10009" />
  <reg:hasSubproperty rdf:resource="http://rdaregistry.info/Elements/p/datatype/P70011" />
  <rdfs:subPropertyOf rdf:resource="http://rdaregistry.info/Elements/p/P70013" />
  <reg:name xml:lang="da">relateretPeriode</reg:name>
  <rdfs:label xml:lang="da">har relateret periode (sted)</rdfs:label>
  <reg:lexicalAlias rdf:resource="http://rdaregistry.info/Elements/p/relateretPeriode.da" />
  <skos:definition xml:lang="da">Relaterer et sted til en periode der er knyttet til et beskrevet sted.</skos:definition>
  <reg:name xml:lang="vi">địaĐiểmKhungThờiGianCóLiênQuan</reg:name>
  <rdfs:label xml:lang="vi">có khung thời gian có liên quan (địa điểm)</rdfs:label>
  <skos:definition xml:lang="vi">Liên kết địa điểm với khung thời gian liên quan tới địa điểm đang được mô tả.</skos:definition>
  <rdfs:label xml:lang="ca">té com a període de temps relacionat (lloc)</rdfs:label>
  <skos:definition xml:lang="ca">Relaciona un lloc amb un període de temps associat amb un lloc que es descriu.</skos:definition>
  <reg:name xml:lang="fi">paikkaanLiittyvaAjankohta</reg:name>
  <rdfs:label xml:lang="fi">paikkaan liittyvä ajankohta</rdfs:label>
  <reg:lexicalAlias rdf:resource="http://rdaregistry.info/Elements/p/paikkaanLiittyvaAjankohta.fi" />
  <skos:definition xml:lang="fi">Liittää paikan ajankohtaan, johon kuvailun kohteena oleva paikka liittyy.</skos:definition>
  <reg:name xml:lang="fr">lapsDeTempsEnRelationLieu</reg:name>
  <rdfs:label xml:lang="fr">a pour laps de temps en relation (lieu)</rdfs:label>
  <reg:lexicalAlias rdf:resource="http://rdaregistry.info/Elements/p/lapsDeTempsEnRelationLieu.fr" />
  <skos:definition xml:lang="fr">Met un lieu en relation avec un laps de temps associé à un lieu décrit.</skos:definition>
  <reg:name xml:lang="el">σχετικόΧρονικόΔιάστημαΤόπος</reg:name>
  <rdfs:label xml:lang="el">έχει σχετικό χρονικό διάστημα (τόπος)</rdfs:label>
  <reg:lexicalAlias rdf:resource="http://rdaregistry.info/Elements/p/σχετικόΧρονικόΔιάστημαΤόπος.el" />
  <skos:definition xml:lang="el">Συνδέει έναν τόπο με ένα χρονικό διάστημα που συνδέεται με έναν περιγραφόμενο τόπο.</skos:definition>
  <rdakit:toolkitLabel xml:lang="en">related timespan of place</rdakit:toolkitLabel>
  <rdakit:toolkitDefinition xml:lang="en">A timespan that is associated with a place.</rdakit:toolkitDefinition>
  <rdakit:hasElementType xml:lang="">1</rdakit:hasElementType>
  <rdfs:subPropertyOf rdf:resource="http://rdaregistry.info/Elements/x/P00011" />
  <reg:name xml:lang="hu">kapcsolódóIdőtartamHely</reg:name>
  <rdfs:label xml:lang="hu">van kapcsolódó időtartama (hely)</rdfs:label>
  <skos:definition xml:lang="hu">Egy helyet hozzákapcsol egy időtartamhoz, amely kötődik egy éppen leírt helyhez.</skos:definition>
  <reg:hasUnconstrained rdf:resource="http://rdaregistry.info/Elements/u/P61019" />
</rdf:Description>

<!-- Property: has related expression of place -->
<rdf:Description rdf:about="http://rdaregistry.info/Elements/p/P70005">
  <rdfs:isDefinedBy rdf:resource="http://rdaregistry.info/Elements/p/" />
  <reg:status rdf:resource="http://metadataregistry.org/uri/RegStatus/1001" />
  <rdf:type rdf:resource="http://www.w3.org/1999/02/22-rdf-syntax-ns#Property" />
  <reg:name xml:lang="en">relatedExpressionOfPlace</reg:name>
  <rdfs:label xml:lang="en">has related expression of place</rdfs:label>
  <reg:lexicalAlias rdf:resource="http://rdaregistry.info/Elements/p/relatedExpressionOfPlace.en" />
  <skos:definition xml:lang="en">Relates a place to an expression that is associated with a place.</skos:definition>
  <rdfs:domain rdf:resource="http://rdaregistry.info/Elements/c/C10009" />
  <reg:hasSubproperty rdf:resource="http://rdaregistry.info/Elements/p/datatype/P70005" />
  <rdfs:subPropertyOf rdf:resource="http://rdaregistry.info/Elements/p/P70013" />
  <reg:name xml:lang="da">relateretUdtrykSted</reg:name>
  <rdfs:label xml:lang="da">har relateret udtryk (sted)</rdfs:label>
  <reg:lexicalAlias rdf:resource="http://rdaregistry.info/Elements/p/relateretUdtrykSted.da" />
  <skos:definition xml:lang="da">Relaterer et sted til et udtryk der er knyttet til et beskrevet sted.</skos:definition>
  <reg:name xml:lang="vi">địaĐiểmBiểuHiệnCóLiênQuan</reg:name>
  <rdfs:label xml:lang="vi">có biểu hiện có liên quan (địa điểm)</rdfs:label>
  <skos:definition xml:lang="vi">Liên kết địa điểm với biểu hiện liên quan tới địa điểm đang được mô tả.</skos:definition>
  <rdfs:label xml:lang="ca">té com a expressió relacionada (lloc)</rdfs:label>
  <skos:definition xml:lang="ca">Relaciona un lloc amb una expressió associada amb un lloc que es descriu.</skos:definition>
  <reg:name xml:lang="fi">paikkaanLiittyvaEkspressio</reg:name>
  <rdfs:label xml:lang="fi">paikkaan liittyvä ekspressio</rdfs:label>
  <reg:lexicalAlias rdf:resource="http://rdaregistry.info/Elements/p/paikkaanLiittyvaEkspressio.fi" />
  <skos:definition xml:lang="fi">Liittää paikan ekspressioon, johon kuvailun kohteena oleva paikka liittyy.</skos:definition>
  <reg:name xml:lang="fr">expressionEnRelationLieu</reg:name>
  <rdfs:label xml:lang="fr">a pour expression en relation (lieu)</rdfs:label>
  <reg:lexicalAlias rdf:resource="http://rdaregistry.info/Elements/p/expressionEnRelationLieu.fr" />
  <skos:definition xml:lang="fr">Met un lieu en relation avec une expression associée à un lieu décrit.</skos:definition>
  <reg:name xml:lang="el">σχετικήΈκφρασηΤόπος</reg:name>
  <rdfs:label xml:lang="el">έχει σχετική έκφραση (τόπος)</rdfs:label>
  <reg:lexicalAlias rdf:resource="http://rdaregistry.info/Elements/p/σχετικήΈκφρασηΤόπος.el" />
  <skos:definition xml:lang="el">Συνδέει έναν τόπο με μια έκφραση που συνδέεται με έναν περιγραφόμενο τόπο.</skos:definition>
  <rdakit:toolkitLabel xml:lang="en">related expression of place</rdakit:toolkitLabel>
  <rdakit:toolkitDefinition xml:lang="en">An expression that is associated with a place.</rdakit:toolkitDefinition>
  <rdakit:hasElementType xml:lang="">1</rdakit:hasElementType>
  <rdfs:subPropertyOf rdf:resource="http://rdaregistry.info/Elements/x/P00003" />
  <reg:name xml:lang="hu">kapcsolódóKifejezésiformaHely</reg:name>
  <rdfs:label xml:lang="hu">van kapcsolódó kifejezési formája (hely)</rdfs:label>
  <skos:definition xml:lang="hu">Egy helyet hozzákapcsol egy kifejezési formához, amely kötődik egy éppen leírt helyhez.</skos:definition>
  <reg:hasSubproperty rdf:resource="http://rdaregistry.info/Elements/p/P70038" />
  <reg:hasUnconstrained rdf:resource="http://rdaregistry.info/Elements/u/P61013" />
</rdf:Description>

<!-- Property: has related collective agent of place -->
<rdf:Description rdf:about="http://rdaregistry.info/Elements/p/P70009">
  <rdfs:isDefinedBy rdf:resource="http://rdaregistry.info/Elements/p/" />
  <reg:status rdf:resource="http://metadataregistry.org/uri/RegStatus/1001" />
  <rdf:type rdf:resource="http://www.w3.org/1999/02/22-rdf-syntax-ns#Property" />
  <reg:name xml:lang="en">relatedCollectiveAgentOfPlace</reg:name>
  <rdfs:label xml:lang="en">has related collective agent of place</rdfs:label>
  <reg:lexicalAlias rdf:resource="http://rdaregistry.info/Elements/p/relatedCollectiveAgentOfPlace.en" />
  <skos:definition xml:lang="en">Relates a place to a collective agent who is associated with a place.</skos:definition>
  <rdfs:domain rdf:resource="http://rdaregistry.info/Elements/c/C10009" />
  <reg:hasSubproperty rdf:resource="http://rdaregistry.info/Elements/p/datatype/P70009" />
  <rdfs:subPropertyOf rdf:resource="http://rdaregistry.info/Elements/p/P70008" />
  <reg:hasSubproperty rdf:resource="http://rdaregistry.info/Elements/p/P70015" />
  <reg:hasSubproperty rdf:resource="http://rdaregistry.info/Elements/p/P70016" />
  <reg:name xml:lang="da">relateretFællesAgentSted</reg:name>
  <rdfs:label xml:lang="da">har relateret kollektiv agent (sted)</rdfs:label>
  <reg:lexicalAlias rdf:resource="http://rdaregistry.info/Elements/p/relateretFællesAgentSted.da" />
  <skos:definition xml:lang="da">Relaterer et sted til en fælles agent der er knyttet til et beskrevet sted.</skos:definition>
  <reg:name xml:lang="vi">địaĐiểmTácNhânTậpThểCóLiênQuan</reg:name>
  <rdfs:label xml:lang="vi">có tác nhân tập thể có liên quan (địa điểm)</rdfs:label>
  <skos:definition xml:lang="vi">Liên kết địa điểm với tác nhân tập thể liên quan tới địa điểm đang được mô tả.</skos:definition>
  <rdfs:label xml:lang="ca">té com a agent col·lectiu relacionat (lloc)</rdfs:label>
  <skos:definition xml:lang="ca">Relaciona un lloc amb un agent col·lectiu associat amb un lloc que es descriu.</skos:definition>
  <reg:name xml:lang="fi">paikkaanLiittyvaYhteistoimija</reg:name>
  <rdfs:label xml:lang="fi">paikkaan liittyvä yhteistoimija</rdfs:label>
  <reg:lexicalAlias rdf:resource="http://rdaregistry.info/Elements/p/paikkaanLiittyvaYhteistoimija.fi" />
  <skos:definition xml:lang="fi">Liittää paikan yhteistoimijaan, johon kuvailun kohteena oleva paikka liittyy.</skos:definition>
  <reg:name xml:lang="fr">agentCollectifEnRelationLieu</reg:name>
  <rdfs:label xml:lang="fr">a pour agent collectif en relation (lieu)</rdfs:label>
  <reg:lexicalAlias rdf:resource="http://rdaregistry.info/Elements/p/agentCollectifEnRelationLieu.fr" />
  <skos:definition xml:lang="fr">Met un lieu en relation avec un agent collectif associé à un lieu décrit.</skos:definition>
  <reg:name xml:lang="el">σχετικόςΣυλλογικόςΦορέαςΤόπος</reg:name>
  <rdfs:label xml:lang="el">έχει σχετικό συλλογικό φορέα (τόπος)</rdfs:label>
  <reg:lexicalAlias rdf:resource="http://rdaregistry.info/Elements/p/σχετικόςΣυλλογικόςΦορέαςΤόπος.el" />
  <skos:definition xml:lang="el">Συνδέει έναν τόπο με έναν συλλογικό φορέα που συνδέεται με έναν περιγραφόμενο τόπο.</skos:definition>
  <rdakit:toolkitLabel xml:lang="en">related collective agent of place</rdakit:toolkitLabel>
  <rdakit:toolkitDefinition xml:lang="en">A collective agent who is associated with a place.</rdakit:toolkitDefinition>
  <rdakit:hasElementType xml:lang="">1</rdakit:hasElementType>
  <rdfs:subPropertyOf rdf:resource="http://rdaregistry.info/Elements/x/P00012" />
  <reg:name xml:lang="hu">kapcsolódóKollektívÁgensHely</reg:name>
  <rdfs:label xml:lang="hu">van kapcsolódó kollektív ágense (hely)</rdfs:label>
  <skos:definition xml:lang="hu">Egy helyet hozzákapcsol egy kollektív ágenshez, amely kötődik egy éppen leírt helyhez.</skos:definition>
  <reg:hasUnconstrained rdf:resource="http://rdaregistry.info/Elements/u/P61011" />
</rdf:Description>

<!-- Property: has related manifestation of place -->
<rdf:Description rdf:about="http://rdaregistry.info/Elements/p/P70006">
  <rdfs:isDefinedBy rdf:resource="http://rdaregistry.info/Elements/p/" />
  <reg:status rdf:resource="http://metadataregistry.org/uri/RegStatus/1001" />
  <rdf:type rdf:resource="http://www.w3.org/1999/02/22-rdf-syntax-ns#Property" />
  <reg:name xml:lang="en">relatedManifestationOfPlace</reg:name>
  <rdfs:label xml:lang="en">has related manifestation of place</rdfs:label>
  <reg:lexicalAlias rdf:resource="http://rdaregistry.info/Elements/p/relatedManifestationOfPlace.en" />
  <skos:definition xml:lang="en">Relates a place to a manifestation that is associated with a place.</skos:definition>
  <rdfs:domain rdf:resource="http://rdaregistry.info/Elements/c/C10009" />
  <reg:hasSubproperty rdf:resource="http://rdaregistry.info/Elements/p/datatype/P70006" />
  <rdfs:subPropertyOf rdf:resource="http://rdaregistry.info/Elements/p/P70013" />
  <reg:name xml:lang="da">relateretManifestationSted</reg:name>
  <rdfs:label xml:lang="da">har relateret manifestation (sted)</rdfs:label>
  <reg:lexicalAlias rdf:resource="http://rdaregistry.info/Elements/p/relateretManifestationSted.da" />
  <skos:definition xml:lang="da">Relaterer et sted til en manifestation der er knyttet til et beskrevet sted.</skos:definition>
  <reg:name xml:lang="vi">địaĐiểmBiểuThịCóLiênQuan</reg:name>
  <rdfs:label xml:lang="vi">có biểu thị có liên quan (địa điểm)</rdfs:label>
  <skos:definition xml:lang="vi">Liên kết địa điểm với biểu thị liên quan tới địa điểm đang được mô tả.</skos:definition>
  <rdfs:label xml:lang="ca">té com a manifestació relacionada (lloc)</rdfs:label>
  <skos:definition xml:lang="ca">Relaciona un lloc amb una manifestació associada amb un lloc que es descriu.</skos:definition>
  <reg:name xml:lang="fi">paikkaanLiittyvaManifestaatio</reg:name>
  <rdfs:label xml:lang="fi">paikkaan liittyvä manifestaatio</rdfs:label>
  <reg:lexicalAlias rdf:resource="http://rdaregistry.info/Elements/p/paikkaanLiittyvaManifestaatio.fi" />
  <skos:definition xml:lang="fi">Liittää paikan manifestaatioon, johon kuvailun kohteena oleva paikka liittyy.</skos:definition>
  <reg:name xml:lang="fr">manifestationEnRelationLieu</reg:name>
  <rdfs:label xml:lang="fr">a pour manifestation en relation (lieu)</rdfs:label>
  <reg:lexicalAlias rdf:resource="http://rdaregistry.info/Elements/p/manifestationEnRelationLieu.fr" />
  <skos:definition xml:lang="fr">Met un lieu en relation avec une manifestation associée à un lieu décrit.</skos:definition>
  <reg:name xml:lang="el">σχετικήΕκδήλωσηΤόπος</reg:name>
  <rdfs:label xml:lang="el">έχει σχετική εκδήλωση (τόπος)</rdfs:label>
  <reg:lexicalAlias rdf:resource="http://rdaregistry.info/Elements/p/σχετικήΕκδήλωσηΤόπος.el" />
  <skos:definition xml:lang="el">Συνδέει έναν τόπο με μια εκδήλωση που συνδέεται με έναν περιγραφόμενο τόπο.</skos:definition>
  <rdakit:toolkitLabel xml:lang="en">related manifestation of place</rdakit:toolkitLabel>
  <rdakit:toolkitDefinition xml:lang="en">A manifestation that is associated with a place.</rdakit:toolkitDefinition>
  <rdakit:hasElementType xml:lang="">1</rdakit:hasElementType>
  <rdfs:subPropertyOf rdf:resource="http://rdaregistry.info/Elements/x/P00004" />
  <reg:name xml:lang="hu">kapcsolódóMegjelenésiformaHely</reg:name>
  <rdfs:label xml:lang="hu">van kapcsolódó megjelenési formája (hely)</rdfs:label>
  <skos:definition xml:lang="hu">Egy helyet hozzákapcsol egy megjelenési formához, amely kötődik egy éppen leírt helyhez.</skos:definition>
  <reg:hasSubproperty rdf:resource="http://rdaregistry.info/Elements/p/P70021" />
  <reg:hasUnconstrained rdf:resource="http://rdaregistry.info/Elements/u/P61013" />
</rdf:Description>

<!-- Property: has related work of place -->
<rdf:Description rdf:about="http://rdaregistry.info/Elements/p/P70004">
  <rdfs:isDefinedBy rdf:resource="http://rdaregistry.info/Elements/p/" />
  <reg:status rdf:resource="http://metadataregistry.org/uri/RegStatus/1001" />
  <rdf:type rdf:resource="http://www.w3.org/1999/02/22-rdf-syntax-ns#Property" />
  <reg:name xml:lang="en">relatedWorkOfPlace</reg:name>
  <rdfs:label xml:lang="en">has related work of place</rdfs:label>
  <reg:lexicalAlias rdf:resource="http://rdaregistry.info/Elements/p/relatedWorkOfPlace.en" />
  <skos:definition xml:lang="en">Relates a place to a work that is associated with a place.</skos:definition>
  <rdfs:domain rdf:resource="http://rdaregistry.info/Elements/c/C10009" />
  <reg:hasSubproperty rdf:resource="http://rdaregistry.info/Elements/p/datatype/P70004" />
  <rdfs:subPropertyOf rdf:resource="http://rdaregistry.info/Elements/p/P70013" />
  <reg:hasSubproperty rdf:resource="http://rdaregistry.info/Elements/p/object/P70004" />
  <reg:name xml:lang="da">relateretVærkSted</reg:name>
  <rdfs:label xml:lang="da">har relateret værk (sted)</rdfs:label>
  <reg:lexicalAlias rdf:resource="http://rdaregistry.info/Elements/p/relateretVærkSted.da" />
  <skos:definition xml:lang="da">Relaterer et sted til et værk der er knyttet til et beskrevet sted.</skos:definition>
  <reg:name xml:lang="vi">địaĐiểmTácPhẩmCóLiênQuan</reg:name>
  <rdfs:label xml:lang="vi">có tác phẩm có liên quan (địa điểm)</rdfs:label>
  <skos:definition xml:lang="vi">Liên kết địa điểm với tác phẩm liên quan tới địa điểm đang được mô tả.</skos:definition>
  <rdfs:label xml:lang="ca">té com a obra relacionada (lloc)</rdfs:label>
  <skos:definition xml:lang="ca">Relaciona un lloc amb una obra associada amb un lloc que es descriu.</skos:definition>
  <reg:name xml:lang="fi">paikkaanLiittyvaTeos</reg:name>
  <rdfs:label xml:lang="fi">paikkaan liittyvä teos</rdfs:label>
  <reg:lexicalAlias rdf:resource="http://rdaregistry.info/Elements/p/paikkaanLiittyvaTeos.fi" />
  <skos:definition xml:lang="fi">Liittää paikan teokseen, johon kuvailun kohteena oleva paikka liittyy.</skos:definition>
  <reg:name xml:lang="fr">œuvreEnRelationLieu</reg:name>
  <rdfs:label xml:lang="fr">a pour œuvre en relation (lieu)</rdfs:label>
  <reg:lexicalAlias rdf:resource="http://rdaregistry.info/Elements/p/œuvreEnRelationLieu.fr" />
  <skos:definition xml:lang="fr">Met un lieu en relation avec une œuvre associée à un lieu décrit.</skos:definition>
  <reg:name xml:lang="el">σχετικόΈργοΤόπος</reg:name>
  <rdfs:label xml:lang="el">έχει σχετικό έργο (τόπος)</rdfs:label>
  <reg:lexicalAlias rdf:resource="http://rdaregistry.info/Elements/p/σχετικόΈργοΤόπος.el" />
  <skos:definition xml:lang="el">Συνδέει έναν τόπο με ένα έργο που συνδέεται με έναν περιγραφόμενο τόπο.</skos:definition>
  <rdakit:toolkitLabel xml:lang="en">related work of place</rdakit:toolkitLabel>
  <rdakit:toolkitDefinition xml:lang="en">A work that is associated with a place.</rdakit:toolkitDefinition>
  <rdakit:hasElementType xml:lang="">1</rdakit:hasElementType>
  <rdfs:subPropertyOf rdf:resource="http://rdaregistry.info/Elements/x/P00002" />
  <reg:name xml:lang="hu">kapcsolódóMűHely</reg:name>
  <rdfs:label xml:lang="hu">van kapcsolódó műve (hely)</rdfs:label>
  <skos:definition xml:lang="hu">Egy helyet hozzákapcsol egy műhöz, amely kötődik egy éppen leírt helyhez.</skos:definition>
  <reg:hasSubproperty rdf:resource="http://rdaregistry.info/Elements/p/P70052" />
  <reg:hasSubproperty rdf:resource="http://rdaregistry.info/Elements/p/P70023" />
  <reg:hasSubproperty rdf:resource="http://rdaregistry.info/Elements/p/P70035" />
  <reg:hasUnconstrained rdf:resource="http://rdaregistry.info/Elements/u/P61013" />
</rdf:Description>

<!-- Property: has related nomen of place -->
<rdf:Description rdf:about="http://rdaregistry.info/Elements/p/P70012">
  <rdfs:isDefinedBy rdf:resource="http://rdaregistry.info/Elements/p/" />
  <reg:status rdf:resource="http://metadataregistry.org/uri/RegStatus/1001" />
  <rdf:type rdf:resource="http://www.w3.org/1999/02/22-rdf-syntax-ns#Property" />
  <reg:name xml:lang="en">relatedNomenOfPlace</reg:name>
  <rdfs:label xml:lang="en">has related nomen of place</rdfs:label>
  <reg:lexicalAlias rdf:resource="http://rdaregistry.info/Elements/p/relatedNomenOfPlace.en" />
  <skos:definition xml:lang="en">Relates a place to a nomen that is associated with a place.</skos:definition>
  <rdfs:domain rdf:resource="http://rdaregistry.info/Elements/c/C10009" />
  <reg:hasSubproperty rdf:resource="http://rdaregistry.info/Elements/p/datatype/P70012" />
  <rdfs:subPropertyOf rdf:resource="http://rdaregistry.info/Elements/p/P70013" />
  <reg:name xml:lang="da">relateretNomenSted</reg:name>
  <rdfs:label xml:lang="da">har relateret nomen (sted)</rdfs:label>
  <reg:lexicalAlias rdf:resource="http://rdaregistry.info/Elements/p/relateretNomenSted.da" />
  <skos:definition xml:lang="da">Relaterer et sted til et nomen der er knyttet til et beskrevet sted.</skos:definition>
  <reg:name xml:lang="vi">địaĐiểmDanhPhápCóLiênQuan</reg:name>
  <rdfs:label xml:lang="vi">có danh pháp có liên quan (địa điểm)</rdfs:label>
  <skos:definition xml:lang="vi">Liên kết địa điểm với danh pháp liên quan tới địa điểm đang được mô tả.</skos:definition>
  <rdfs:label xml:lang="ca">té com a nomen relacionat (lloc)</rdfs:label>
  <skos:definition xml:lang="ca">Relaciona un lloc amb un nomen associat amb un lloc que es descriu.</skos:definition>
  <reg:name xml:lang="fi">paikkaanLiittyvaNomen</reg:name>
  <rdfs:label xml:lang="fi">paikkaan liittyvä nomen</rdfs:label>
  <reg:lexicalAlias rdf:resource="http://rdaregistry.info/Elements/p/paikkaanLiittyvaNomen.fi" />
  <skos:definition xml:lang="fi">Liittää paikan nomeniin, johon kuvailun kohteena oleva paikka liittyy.</skos:definition>
  <reg:name xml:lang="fr">nomenEnRelationLieu</reg:name>
  <rdfs:label xml:lang="fr">a pour nomen en relation (lieu)</rdfs:label>
  <reg:lexicalAlias rdf:resource="http://rdaregistry.info/Elements/p/nomenEnRelationLieu.fr" />
  <skos:definition xml:lang="fr">Met un lieu en relation avec un nomen associé à un lieu décrit.</skos:definition>
  <reg:name xml:lang="el">σχετικόΌνομαΤόπου</reg:name>
  <rdfs:label xml:lang="el">έχει σχετικό όνομα (τόπος)</rdfs:label>
  <reg:lexicalAlias rdf:resource="http://rdaregistry.info/Elements/p/σχετικόΌνομαΤόπου.el" />
  <skos:definition xml:lang="el">Συνδέει έναν τόπο με ένα όνομα που συνδέεται με έναν περιγραφόμενο τόπο.</skos:definition>
  <rdakit:toolkitLabel xml:lang="en">related nomen of place</rdakit:toolkitLabel>
  <rdakit:toolkitDefinition xml:lang="en">A nomen that is associated with a place.</rdakit:toolkitDefinition>
  <rdakit:hasElementType xml:lang="">1</rdakit:hasElementType>
  <rdfs:subPropertyOf rdf:resource="http://rdaregistry.info/Elements/x/P00013" />
  <reg:name xml:lang="hu">kapcsolódóNomenHely</reg:name>
  <rdfs:label xml:lang="hu">van kapcsolódó nomene (hely)</rdfs:label>
  <skos:definition xml:lang="hu">Egy helyet hozzákapcsol egy nomenhez, amely kötődik egy éppen leírt helyhez.</skos:definition>
  <reg:hasSubproperty rdf:resource="http://rdaregistry.info/Elements/p/P70019" />
  <reg:hasUnconstrained rdf:resource="http://rdaregistry.info/Elements/u/P61025" />
</rdf:Description>

<!-- Property: has related item of place -->
<rdf:Description rdf:about="http://rdaregistry.info/Elements/p/P70007">
  <rdfs:isDefinedBy rdf:resource="http://rdaregistry.info/Elements/p/" />
  <reg:status rdf:resource="http://metadataregistry.org/uri/RegStatus/1001" />
  <rdf:type rdf:resource="http://www.w3.org/1999/02/22-rdf-syntax-ns#Property" />
  <reg:name xml:lang="en">relatedItemOfPlace</reg:name>
  <rdfs:label xml:lang="en">has related item of place</rdfs:label>
  <reg:lexicalAlias rdf:resource="http://rdaregistry.info/Elements/p/relatedItemOfPlace.en" />
  <skos:definition xml:lang="en">Relates a place to an item that is associated with a place.</skos:definition>
  <rdfs:domain rdf:resource="http://rdaregistry.info/Elements/c/C10009" />
  <reg:hasSubproperty rdf:resource="http://rdaregistry.info/Elements/p/datatype/P70007" />
  <rdfs:subPropertyOf rdf:resource="http://rdaregistry.info/Elements/p/P70013" />
  <reg:name xml:lang="da">relateretEksemplarSted</reg:name>
  <rdfs:label xml:lang="da">har relateret eksemplar (sted)</rdfs:label>
  <reg:lexicalAlias rdf:resource="http://rdaregistry.info/Elements/p/relateretEksemplarSted.da" />
  <skos:definition xml:lang="da">Relaterer et sted til et eksemplar der er knyttet til et beskrevet sted.</skos:definition>
  <reg:name xml:lang="vi">địaĐiểmBảnCóLiênQuan</reg:name>
  <rdfs:label xml:lang="vi">có bản có liên quan (địa điểm)</rdfs:label>
  <skos:definition xml:lang="vi">Liên kết địa điểm với bản liên quan tới địa điểm đang được mô tả.</skos:definition>
  <rdfs:label xml:lang="ca">té com a ítem relacionat (lloc)</rdfs:label>
  <skos:definition xml:lang="ca">Relaciona un lloc amb una obra associada amb un lloc que es descriu.</skos:definition>
  <reg:name xml:lang="fi">paikkaanLiittyvaKappale</reg:name>
  <rdfs:label xml:lang="fi">paikkaan liittyvä kappale</rdfs:label>
  <reg:lexicalAlias rdf:resource="http://rdaregistry.info/Elements/p/paikkaanLiittyvaKappale.fi" />
  <skos:definition xml:lang="fi">Liittää paikan kappaleeseen, johon kuvailun kohteena oleva paikka liittyy.</skos:definition>
  <reg:name xml:lang="fr">itemEnRelationLieu</reg:name>
  <rdfs:label xml:lang="fr">a pour item en relation (lieu)</rdfs:label>
  <reg:lexicalAlias rdf:resource="http://rdaregistry.info/Elements/p/itemEnRelationLieu.fr" />
  <skos:definition xml:lang="fr">Met un lieu en relation avec un item associé à un lieu décrit.</skos:definition>
  <reg:name xml:lang="el">σχετικόΑντίτυποΤόπος</reg:name>
  <rdfs:label xml:lang="el">έχει σχετικό αντίτυπο (τόπος)</rdfs:label>
  <reg:lexicalAlias rdf:resource="http://rdaregistry.info/Elements/p/σχετικόΑντίτυποΤόπος.el" />
  <skos:definition xml:lang="el">Συνδέει έναν τόπο με ένα αντίτυπο που συνδέεται με έναν περιγραφόμενο τόπο.</skos:definition>
  <rdakit:toolkitLabel xml:lang="en">related item of place</rdakit:toolkitLabel>
  <rdakit:toolkitDefinition xml:lang="en">An item that is associated with a place.</rdakit:toolkitDefinition>
  <rdakit:hasElementType xml:lang="">1</rdakit:hasElementType>
  <rdfs:subPropertyOf rdf:resource="http://rdaregistry.info/Elements/x/P00005" />
  <reg:name xml:lang="hu">kapcsolódóPéldányHely</reg:name>
  <rdfs:label xml:lang="hu">van kapcsolódó példánya (hely)</rdfs:label>
  <skos:definition xml:lang="hu">Egy helyet hozzákapcsol egy példányhoz, amely kötődik egy éppen leírt helyhez.</skos:definition>
  <reg:hasUnconstrained rdf:resource="http://rdaregistry.info/Elements/u/P61013" />
</rdf:Description>

<!-- Property: has related person of place -->
<rdf:Description rdf:about="http://rdaregistry.info/Elements/p/P70014">
  <rdfs:isDefinedBy rdf:resource="http://rdaregistry.info/Elements/p/" />
  <reg:status rdf:resource="http://metadataregistry.org/uri/RegStatus/1001" />
  <rdfs:subPropertyOf rdf:resource="http://rdaregistry.info/Elements/p/P70008" />
  <rdf:type rdf:resource="http://www.w3.org/1999/02/22-rdf-syntax-ns#Property" />
  <reg:name xml:lang="en">relatedPersonOfPlace</reg:name>
  <rdfs:label xml:lang="en">has related person of place</rdfs:label>
  <reg:lexicalAlias rdf:resource="http://rdaregistry.info/Elements/p/relatedPersonOfPlace.en" />
  <skos:definition xml:lang="en">Relates a place to a person who is associated with a place.</skos:definition>
  <rdfs:domain rdf:resource="http://rdaregistry.info/Elements/c/C10009" />
  <reg:hasSubproperty rdf:resource="http://rdaregistry.info/Elements/p/P70014" />
  <reg:hasSubproperty rdf:resource="http://rdaregistry.info/Elements/p/datatype/P70014" />
  <reg:name xml:lang="da">relateretPersonSted</reg:name>
  <rdfs:label xml:lang="da">har relateret person (sted)</rdfs:label>
  <reg:lexicalAlias rdf:resource="http://rdaregistry.info/Elements/p/relateretPersonSted.da" />
  <skos:definition xml:lang="da">Relaterer et sted til en person der er knyttet til et beskrevet sted.</skos:definition>
  <reg:name xml:lang="vi">địaĐiểmCáNhânCóLiênQuan</reg:name>
  <rdfs:label xml:lang="vi">có cá nhân có liên quan (địa điểm)</rdfs:label>
  <skos:definition xml:lang="vi">Liên kết địa điểm với cá nhân liên quan tới địa điểm đang được mô tả.</skos:definition>
  <rdfs:label xml:lang="ca">té com a persona relacionada (lloc)</rdfs:label>
  <skos:definition xml:lang="ca">Relaciona un lloc amb una persona associada amb un lloc que es descriu.</skos:definition>
  <reg:name xml:lang="fi">paikkaanLiittyvaHenkilo</reg:name>
  <rdfs:label xml:lang="fi">paikkaan liittyvä henkilö</rdfs:label>
  <reg:lexicalAlias rdf:resource="http://rdaregistry.info/Elements/p/paikkaanLiittyvaHenkilo.fi" />
  <skos:definition xml:lang="fi">Liittää paikan henkilöön, johon kuvailun kohteena oleva paikka liittyy.</skos:definition>
  <reg:name xml:lang="fr">personneEnRelationLieu</reg:name>
  <rdfs:label xml:lang="fr">a pour personne en relation (lieu)</rdfs:label>
  <reg:lexicalAlias rdf:resource="http://rdaregistry.info/Elements/p/personneEnRelationLieu.fr" />
  <skos:definition xml:lang="fr">Met un lieu en relation avec une personne associée à un lieu décrit.</skos:definition>
  <reg:name xml:lang="el">σχετικόΦυσικόΠρόσωποΤόπος</reg:name>
  <rdfs:label xml:lang="el">έχει σχετικό φυσικό πρόσωπο (τόπος)</rdfs:label>
  <reg:lexicalAlias rdf:resource="http://rdaregistry.info/Elements/p/σχετικόΦυσικόΠρόσωποΤόπος.el" />
  <skos:definition xml:lang="el">Συνδέει έναν τόπο με ένα φυσικό πρόσωπο που συνδέεται με έναν περιγραφόμενο τόπο.</skos:definition>
  <rdakit:toolkitLabel xml:lang="en">related person of place</rdakit:toolkitLabel>
  <rdakit:toolkitDefinition xml:lang="en">A person who is associated with a place.</rdakit:toolkitDefinition>
  <rdakit:hasElementType xml:lang="">1</rdakit:hasElementType>
  <rdfs:subPropertyOf rdf:resource="http://rdaregistry.info/Elements/x/P00007" />
  <reg:name xml:lang="hu">kapcsolódóSzemélyHely</reg:name>
  <rdfs:label xml:lang="hu">van kapcsolódó személye (hely)</rdfs:label>
  <skos:definition xml:lang="hu">Egy helyet hozzákapcsol egy személyhez, aki kötődik egy éppen leírt helyhez.</skos:definition>
  <reg:hasSubproperty rdf:resource="http://rdaregistry.info/Elements/p/P70025" />
  <reg:hasSubproperty rdf:resource="http://rdaregistry.info/Elements/p/P70026" />
  <reg:hasSubproperty rdf:resource="http://rdaregistry.info/Elements/p/P70027" />
  <reg:hasUnconstrained rdf:resource="http://rdaregistry.info/Elements/u/P61011" />
</rdf:Description>

<!-- Property: has related corporate body of place -->
<rdf:Description rdf:about="http://rdaregistry.info/Elements/p/P70016">
  <rdfs:isDefinedBy rdf:resource="http://rdaregistry.info/Elements/p/" />
  <reg:status rdf:resource="http://metadataregistry.org/uri/RegStatus/1001" />
  <rdfs:subPropertyOf rdf:resource="http://rdaregistry.info/Elements/p/P70009" />
  <rdf:type rdf:resource="http://www.w3.org/1999/02/22-rdf-syntax-ns#Property" />
  <reg:name xml:lang="en">relatedCorporateBodyOfPlace</reg:name>
  <rdfs:label xml:lang="en">has related corporate body of place</rdfs:label>
  <reg:lexicalAlias rdf:resource="http://rdaregistry.info/Elements/p/relatedCorporateBodyOfPlace.en" />
  <skos:definition xml:lang="en">Relates a place to a corporate body who is associated with a place.</skos:definition>
  <rdfs:domain rdf:resource="http://rdaregistry.info/Elements/c/C10009" />
  <reg:hasSubproperty rdf:resource="http://rdaregistry.info/Elements/p/P70016" />
  <reg:hasSubproperty rdf:resource="http://rdaregistry.info/Elements/p/datatype/P70016" />
  <reg:name xml:lang="da">relateretKorporationSted</reg:name>
  <rdfs:label xml:lang="da">har relateret korporation (sted)</rdfs:label>
  <reg:lexicalAlias rdf:resource="http://rdaregistry.info/Elements/p/relateretKorporationSted.da" />
  <skos:definition xml:lang="da">Relaterer et sted til en korporation der er knyttet til et beskrevet sted.</skos:definition>
  <reg:name xml:lang="vi">địaĐiểmTậpThểCóLiênQuan</reg:name>
  <rdfs:label xml:lang="vi">có tập thể có liên quan (địa điểm)</rdfs:label>
  <skos:definition xml:lang="vi">Liên kết địa điểm với tập thể liên quan tới địa điểm đang được mô tả.</skos:definition>
  <rdfs:label xml:lang="ca">té com a entitat corporativa relacionada (lloc)</rdfs:label>
  <skos:definition xml:lang="ca">Relaciona un lloc amb una entitat corporativa associada amb un lloc que es descriu.</skos:definition>
  <reg:name xml:lang="fi">paikkaanLiittyvaYhteiso</reg:name>
  <rdfs:label xml:lang="fi">paikkaan liittyvä yhteisö</rdfs:label>
  <reg:lexicalAlias rdf:resource="http://rdaregistry.info/Elements/p/paikkaanLiittyvaYhteiso.fi" />
  <skos:definition xml:lang="fi">Liittää paikan yhteisöön, johon kuvailun kohteena oleva paikka liittyy.</skos:definition>
  <reg:name xml:lang="fr">collectivitéEnRelationLieu</reg:name>
  <rdfs:label xml:lang="fr">a pour collectivité en relation (lieu)</rdfs:label>
  <reg:lexicalAlias rdf:resource="http://rdaregistry.info/Elements/p/collectivitéEnRelationLieu.fr" />
  <skos:definition xml:lang="fr">Met un lieu en relation avec une collectivité associée à un lieu décrit.</skos:definition>
  <reg:name xml:lang="el">σχετικόΣυλλογικόΌργανοΤόπος</reg:name>
  <rdfs:label xml:lang="el">έχει σχετικό συλλογικό όργανο (τόπος)</rdfs:label>
  <reg:lexicalAlias rdf:resource="http://rdaregistry.info/Elements/p/σχετικόΣυλλογικόΌργανοΤόπος.el" />
  <skos:definition xml:lang="el">Συνδέει έναν τόπο με ένα συλλογικό όργανο που συνδέεται με έναν περιγραφόμενο τόπο.</skos:definition>
  <rdakit:toolkitLabel xml:lang="en">related corporate body of place</rdakit:toolkitLabel>
  <rdakit:toolkitDefinition xml:lang="en">A corporate body who is associated with a place.</rdakit:toolkitDefinition>
  <rdakit:hasElementType xml:lang="">1</rdakit:hasElementType>
  <reg:hasSubproperty rdf:resource="http://rdaregistry.info/Elements/p/P70051" />
  <rdfs:subPropertyOf rdf:resource="http://rdaregistry.info/Elements/x/P00009" />
  <reg:name xml:lang="hu">kapcsolódóTestületHely</reg:name>
  <rdfs:label xml:lang="hu">van kapcsolódó testülete (hely)</rdfs:label>
  <skos:definition xml:lang="hu">Egy helyet hozzákapcsol egy testülethez, amely kötődik egy éppen leírt helyhez.</skos:definition>
  <skos:altLabel xml:lang="en">place associated with corporate body of</skos:altLabel>
  <reg:hasSubproperty rdf:resource="http://rdaregistry.info/Elements/p/P70028" />
  <reg:hasUnconstrained rdf:resource="http://rdaregistry.info/Elements/u/P61011" />
</rdf:Description>

<!-- Property: has location -->
<rdf:Description rdf:about="http://rdaregistry.info/Elements/p/P70043">
  <rdfs:isDefinedBy rdf:resource="http://rdaregistry.info/Elements/p/" />
  <reg:status rdf:resource="http://metadataregistry.org/uri/RegStatus/1001" />
  <rdf:type rdf:resource="http://www.w3.org/1999/02/22-rdf-syntax-ns#Property" />
  <reg:name xml:lang="en">location</reg:name>
  <rdfs:label xml:lang="en">has location</rdfs:label>
  <reg:lexicalAlias rdf:resource="http://rdaregistry.info/Elements/p/location.en" />
  <skos:definition xml:lang="en">Relates a place to a delimitation of the physical territory of the place.</skos:definition>
  <rdfs:domain rdf:resource="http://rdaregistry.info/Elements/c/C10009" />
  <rdakit:toolkitLabel xml:lang="en">location</rdakit:toolkitLabel>
  <rdakit:toolkitDefinition xml:lang="en">A delimitation of the physical territory of a place.</rdakit:toolkitDefinition>
  <rdakit:hasElementType xml:lang="">6</rdakit:hasElementType>
  <reg:hasSubproperty rdf:resource="http://rdaregistry.info/Elements/p/datatype/P70043" />
</rdf:Description>

<!-- Property: is longitude and latitude of -->
<rdf:Description rdf:about="http://rdaregistry.info/Elements/p/P70034">
  <rdfs:isDefinedBy rdf:resource="http://rdaregistry.info/Elements/p/" />
  <reg:status rdf:resource="http://metadataregistry.org/uri/RegStatus/1001" />
  <rdf:type rdf:resource="http://www.w3.org/1999/02/22-rdf-syntax-ns#Property" />
  <reg:name xml:lang="en">longitudeAndLatitudeOf</reg:name>
  <rdfs:label xml:lang="en">is longitude and latitude of</rdfs:label>
  <reg:lexicalAlias rdf:resource="http://rdaregistry.info/Elements/p/longitudeAndLatitudeOf.en" />
  <rdfs:domain rdf:resource="http://rdaregistry.info/Elements/c/C10009" />
  <rdakit:toolkitLabel xml:lang="en">longitude and latitude of</rdakit:toolkitLabel>
  <reg:hasSubproperty rdf:resource="http://rdaregistry.info/Elements/p/object/P70034" />
  <rdfs:subPropertyOf rdf:resource="http://rdaregistry.info/Elements/p/P70023" />
  <rdakit:hasElementType xml:lang="">2</rdakit:hasElementType>
  <reg:hasSubproperty rdf:resource="http://rdaregistry.info/Elements/p/datatype/P70034" />
  <skos:definition xml:lang="en">Relates a place to a work that is a cartographic work that has an area of coverage that is identified using longitude of the westernmost and easternmost boundaries and latitude of the northernmost and southernmost boundaries.</skos:definition>
  <rdakit:toolkitDefinition xml:lang="en">A work that is a cartographic work that has an area of coverage that is identified using longitude of the westernmost and easternmost boundaries and latitude of the northernmost and southernmost boundaries.</rdakit:toolkitDefinition>
</rdf:Description>

<!-- Property: has note on place -->
<rdf:Description rdf:about="http://rdaregistry.info/Elements/p/P70022">
  <rdfs:isDefinedBy rdf:resource="http://rdaregistry.info/Elements/p/" />
  <reg:status rdf:resource="http://metadataregistry.org/uri/RegStatus/1001" />
  <rdf:type rdf:resource="http://www.w3.org/1999/02/22-rdf-syntax-ns#Property" />
  <reg:name xml:lang="en">noteOnPlace</reg:name>
  <rdfs:label xml:lang="en">has note on place</rdfs:label>
  <reg:lexicalAlias rdf:resource="http://rdaregistry.info/Elements/p/noteOnPlace.en" />
  <skos:definition xml:lang="en">Relates a place to a broad unstructured description of one or more attributes of a place.</skos:definition>
  <rdfs:domain rdf:resource="http://rdaregistry.info/Elements/c/C10009" />
  <rdakit:toolkitLabel xml:lang="en">note on place</rdakit:toolkitLabel>
  <rdakit:toolkitDefinition xml:lang="en">A broad unstructured description of one or more attributes of a place.</rdakit:toolkitDefinition>
  <reg:hasUnconstrained rdf:resource="http://rdaregistry.info/Elements/u/P60936" />
  <rdakit:hasElementType xml:lang="">6</rdakit:hasElementType>
  <rdfs:subPropertyOf rdf:resource="http://rdaregistry.info/Elements/x/P00015" />
  <reg:hasSubproperty rdf:resource="http://rdaregistry.info/Elements/p/datatype/P70022" />
</rdf:Description>

<!-- Property: DEPRECATED -->
<rdf:Description rdf:about="http://rdaregistry.info/Elements/p/P70029">
  <rdfs:isDefinedBy rdf:resource="http://rdaregistry.info/Elements/p/" />
  <reg:status rdf:resource="http://metadataregistry.org/uri/RegStatus/1008" />
  <rdf:type rdf:resource="http://www.w3.org/1999/02/22-rdf-syntax-ns#Property" />
  <reg:name xml:lang="en">otherPlaceAssociatedWithCorporateBodyOf</reg:name>
  <rdfs:label xml:lang="en">is other place associated with corporate body of (Deprecated)</rdfs:label>
  <reg:hasSubproperty rdf:resource="http://rdaregistry.info/Elements/p/object/P70029" />
  <rdakit:hasElementType xml:lang="">3</rdakit:hasElementType>
  <reg:hasSubproperty rdf:resource="http://rdaregistry.info/Elements/p/datatype/P70029" />
</rdf:Description>

<!-- Property: is parallel place of distribution of -->
<rdf:Description rdf:about="http://rdaregistry.info/Elements/p/P70047">
  <rdfs:isDefinedBy rdf:resource="http://rdaregistry.info/Elements/p/" />
  <reg:status rdf:resource="http://metadataregistry.org/uri/RegStatus/1001" />
  <rdfs:label xml:lang="en">is parallel place of distribution of</rdfs:label>
  <rdf:type rdf:resource="http://www.w3.org/1999/02/22-rdf-syntax-ns#Property" />
  <reg:name xml:lang="en">parallelPlaceOfDistributionOf</reg:name>
  <reg:hasSubproperty rdf:resource="http://rdaregistry.info/Elements/p/object/P70047" />
  <rdakit:hasElementType xml:lang="">2</rdakit:hasElementType>
  <reg:hasSubproperty rdf:resource="http://rdaregistry.info/Elements/p/datatype/P70047" />
  <reg:lexicalAlias rdf:resource="http://rdaregistry.info/Elements/p/parallelPlaceOfDistributionOf.en" />
  <skos:definition xml:lang="en">Relates a place to a manifestation that is a published manifestation that is distributed from a place.</skos:definition>
  <rdakit:toolkitLabel xml:lang="en">parallel place of distribution of</rdakit:toolkitLabel>
  <rdakit:toolkitDefinition xml:lang="en">A manifestation that is a published manifestation that is distributed from a place.</rdakit:toolkitDefinition>
  <rdfs:subPropertyOf rdf:resource="http://rdaregistry.info/Elements/p/P70039" />
  <rdfs:domain rdf:resource="http://rdaregistry.info/Elements/c/C10009" />
  <reg:hasUnconstrained rdf:resource="http://rdaregistry.info/Elements/u/P60164" />
</rdf:Description>

<!-- Property: is parallel place of manufacture of -->
<rdf:Description rdf:about="http://rdaregistry.info/Elements/p/P70048">
  <rdfs:isDefinedBy rdf:resource="http://rdaregistry.info/Elements/p/" />
  <reg:status rdf:resource="http://metadataregistry.org/uri/RegStatus/1001" />
  <rdfs:label xml:lang="en">is parallel place of manufacture of</rdfs:label>
  <rdf:type rdf:resource="http://www.w3.org/1999/02/22-rdf-syntax-ns#Property" />
  <reg:name xml:lang="en">parallelPlaceOfManufactureOf</reg:name>
  <reg:hasSubproperty rdf:resource="http://rdaregistry.info/Elements/p/object/P70048" />
  <rdakit:hasElementType xml:lang="">2</rdakit:hasElementType>
  <reg:hasSubproperty rdf:resource="http://rdaregistry.info/Elements/p/datatype/P70048" />
  <reg:lexicalAlias rdf:resource="http://rdaregistry.info/Elements/p/parallelPlaceOfManufactureOf.en" />
  <skos:definition xml:lang="en">Relates a place to a manifestation that is a published manifestation that is printed, duplicated, cast, etc., in a place.</skos:definition>
  <rdakit:toolkitLabel xml:lang="en">parallel place of manufacture of</rdakit:toolkitLabel>
  <rdakit:toolkitDefinition xml:lang="en">A manifestation that is a published manifestation that is printed, duplicated, cast, etc., in a place.</rdakit:toolkitDefinition>
  <rdfs:subPropertyOf rdf:resource="http://rdaregistry.info/Elements/p/P70040" />
  <rdfs:domain rdf:resource="http://rdaregistry.info/Elements/c/C10009" />
  <reg:hasUnconstrained rdf:resource="http://rdaregistry.info/Elements/u/P60165" />
</rdf:Description>

<!-- Property: is parallel place of production of -->
<rdf:Description rdf:about="http://rdaregistry.info/Elements/p/P70049">
  <rdfs:isDefinedBy rdf:resource="http://rdaregistry.info/Elements/p/" />
  <reg:status rdf:resource="http://metadataregistry.org/uri/RegStatus/1001" />
  <rdfs:label xml:lang="en">is parallel place of production of</rdfs:label>
  <rdf:type rdf:resource="http://www.w3.org/1999/02/22-rdf-syntax-ns#Property" />
  <reg:name xml:lang="en">parallelPlaceOfProductionOf</reg:name>
  <reg:hasSubproperty rdf:resource="http://rdaregistry.info/Elements/p/object/P70049" />
  <rdakit:hasElementType xml:lang="">2</rdakit:hasElementType>
  <reg:hasSubproperty rdf:resource="http://rdaregistry.info/Elements/p/datatype/P70049" />
  <reg:lexicalAlias rdf:resource="http://rdaregistry.info/Elements/p/parallelPlaceOfProductionOf.en" />
  <skos:definition xml:lang="en">Relates a place to a manifestation that is an unpublished manifestation that is inscribed, fabricated, constructed, etc., in a place.</skos:definition>
  <rdakit:toolkitLabel xml:lang="en">parallel place of production of</rdakit:toolkitLabel>
  <rdakit:toolkitDefinition xml:lang="en">A manifestation that is an unpublished manifestation that is inscribed, fabricated, constructed, etc., in a place.</rdakit:toolkitDefinition>
  <rdfs:subPropertyOf rdf:resource="http://rdaregistry.info/Elements/p/P70041" />
  <rdfs:domain rdf:resource="http://rdaregistry.info/Elements/c/C10009" />
  <reg:hasUnconstrained rdf:resource="http://rdaregistry.info/Elements/u/P60166" />
</rdf:Description>

<!-- Property: is parallel place of publication of -->
<rdf:Description rdf:about="http://rdaregistry.info/Elements/p/P70050">
  <rdfs:isDefinedBy rdf:resource="http://rdaregistry.info/Elements/p/" />
  <reg:status rdf:resource="http://metadataregistry.org/uri/RegStatus/1001" />
  <rdfs:label xml:lang="en">is parallel place of publication of</rdfs:label>
  <rdf:type rdf:resource="http://www.w3.org/1999/02/22-rdf-syntax-ns#Property" />
  <reg:name xml:lang="en">parallelPlaceOfPublicationOf</reg:name>
  <reg:hasSubproperty rdf:resource="http://rdaregistry.info/Elements/p/object/P70050" />
  <rdakit:hasElementType xml:lang="">2</rdakit:hasElementType>
  <reg:hasSubproperty rdf:resource="http://rdaregistry.info/Elements/p/datatype/P70050" />
  <reg:lexicalAlias rdf:resource="http://rdaregistry.info/Elements/p/parallelPlaceOfPublicationOf.en" />
  <skos:definition xml:lang="en">Relates a place to a manifestation that is a published manifestation that is published, released, or issued in a place.</skos:definition>
  <rdakit:toolkitLabel xml:lang="en">parallel place of publication of</rdakit:toolkitLabel>
  <rdakit:toolkitDefinition xml:lang="en">A manifestation that is a published manifestation that is published, released, or issued in a place.</rdakit:toolkitDefinition>
  <rdfs:subPropertyOf rdf:resource="http://rdaregistry.info/Elements/p/P70042" />
  <rdfs:domain rdf:resource="http://rdaregistry.info/Elements/c/C10009" />
  <reg:hasUnconstrained rdf:resource="http://rdaregistry.info/Elements/u/P60167" />
</rdf:Description>

<!-- Property: is part of place -->
<rdf:Description rdf:about="http://rdaregistry.info/Elements/p/P70032">
  <rdfs:isDefinedBy rdf:resource="http://rdaregistry.info/Elements/p/" />
  <reg:status rdf:resource="http://metadataregistry.org/uri/RegStatus/1001" />
  <rdf:type rdf:resource="http://www.w3.org/1999/02/22-rdf-syntax-ns#Property" />
  <reg:name xml:lang="en">partOfPlace</reg:name>
  <rdfs:label xml:lang="en">is part of place</rdfs:label>
  <reg:lexicalAlias rdf:resource="http://rdaregistry.info/Elements/p/partOfPlace.en" />
  <rdfs:domain rdf:resource="http://rdaregistry.info/Elements/c/C10009" />
  <rdakit:toolkitLabel xml:lang="en">part of place</rdakit:toolkitLabel>
  <reg:hasSubproperty rdf:resource="http://rdaregistry.info/Elements/p/object/P70032" />
  <rdfs:subPropertyOf rdf:resource="http://rdaregistry.info/Elements/p/P70010" />
  <rdakit:hasElementType xml:lang="">2</rdakit:hasElementType>
  <skos:definition xml:lang="en">Relates a place to a place that encompasses another place.</skos:definition>
  <rdakit:toolkitDefinition xml:lang="en">A place that encompasses another place.</rdakit:toolkitDefinition>
  <reg:hasSubproperty rdf:resource="http://rdaregistry.info/Elements/p/datatype/P70032" />
  <reg:hasUnconstrained rdf:resource="http://rdaregistry.info/Elements/u/P61001" />
</rdf:Description>

<!-- Property: has part place -->
<rdf:Description rdf:about="http://rdaregistry.info/Elements/p/P70033">
  <rdfs:isDefinedBy rdf:resource="http://rdaregistry.info/Elements/p/" />
  <reg:status rdf:resource="http://metadataregistry.org/uri/RegStatus/1001" />
  <rdf:type rdf:resource="http://www.w3.org/1999/02/22-rdf-syntax-ns#Property" />
  <reg:name xml:lang="en">partPlace</reg:name>
  <rdfs:label xml:lang="en">has part place</rdfs:label>
  <reg:lexicalAlias rdf:resource="http://rdaregistry.info/Elements/p/partPlace.en" />
  <rdfs:domain rdf:resource="http://rdaregistry.info/Elements/c/C10009" />
  <rdakit:toolkitLabel xml:lang="en">part place</rdakit:toolkitLabel>
  <reg:hasSubproperty rdf:resource="http://rdaregistry.info/Elements/p/object/P70033" />
  <rdfs:subPropertyOf rdf:resource="http://rdaregistry.info/Elements/p/P70010" />
  <rdakit:hasElementType xml:lang="">2</rdakit:hasElementType>
  <skos:definition xml:lang="en">Relates a place to a place that is located within another place.</skos:definition>
  <rdakit:toolkitDefinition xml:lang="en">A place that is located within another place.</rdakit:toolkitDefinition>
  <reg:hasSubproperty rdf:resource="http://rdaregistry.info/Elements/p/datatype/P70033" />
  <reg:hasUnconstrained rdf:resource="http://rdaregistry.info/Elements/u/P61003" />
</rdf:Description>

<!-- Property: DEPRECATED -->
<rdf:Description rdf:about="http://rdaregistry.info/Elements/p/P70030">
  <rdfs:isDefinedBy rdf:resource="http://rdaregistry.info/Elements/p/" />
  <reg:status rdf:resource="http://metadataregistry.org/uri/RegStatus/1008" />
  <rdf:type rdf:resource="http://www.w3.org/1999/02/22-rdf-syntax-ns#Property" />
  <reg:name xml:lang="en">placeAssociatedWithCorporateBodyOf</reg:name>
  <rdfs:label xml:lang="en">is place associated with corporate body of (Deprecated)</rdfs:label>
  <reg:hasSubproperty rdf:resource="http://rdaregistry.info/Elements/p/object/P70030" />
  <rdakit:hasElementType xml:lang="">2</rdakit:hasElementType>
  <reg:hasSubproperty rdf:resource="http://rdaregistry.info/Elements/p/datatype/P70030" />
  <reg:hasSubproperty rdf:resource="http://rdaregistry.info/Elements/p/P70029" />
</rdf:Description>

<!-- Property: DEPRECATED -->
<rdf:Description rdf:about="http://rdaregistry.info/Elements/p/P70031">
  <rdfs:isDefinedBy rdf:resource="http://rdaregistry.info/Elements/p/" />
  <reg:status rdf:resource="http://metadataregistry.org/uri/RegStatus/1008" />
  <rdf:type rdf:resource="http://www.w3.org/1999/02/22-rdf-syntax-ns#Property" />
  <reg:name xml:lang="en">placeAssociatedWithFamilyOf</reg:name>
  <rdfs:label xml:lang="en">is place associated with family of (Deprecated)</rdfs:label>
  <reg:hasSubproperty rdf:resource="http://rdaregistry.info/Elements/p/object/P70031" />
  <rdakit:hasElementType xml:lang="">2</rdakit:hasElementType>
  <reg:hasSubproperty rdf:resource="http://rdaregistry.info/Elements/p/datatype/P70031" />
</rdf:Description>

<!-- Property: is place described in -->
<rdf:Description rdf:about="http://rdaregistry.info/Elements/p/P70054">
  <rdfs:isDefinedBy rdf:resource="http://rdaregistry.info/Elements/p/" />
  <reg:status rdf:resource="http://metadataregistry.org/uri/RegStatus/1001" />
  <rdfs:label xml:lang="en">is place described in</rdfs:label>
  <reg:lexicalAlias rdf:resource="http://rdaregistry.info/Elements/p/placeDescribedIn.en" />
  <skos:definition xml:lang="en">Relates a place to a work that describes a place.</skos:definition>
  <rdakit:toolkitLabel xml:lang="en">place described in</rdakit:toolkitLabel>
  <rdakit:toolkitDefinition xml:lang="en">A work that describes a place.</rdakit:toolkitDefinition>
  <rdf:type rdf:resource="http://www.w3.org/1999/02/22-rdf-syntax-ns#Property" />
  <reg:name xml:lang="">placeDescribedIn</reg:name>
  <rdfs:domain rdf:resource="http://rdaregistry.info/Elements/c/C10009" />
  <rdfs:subPropertyOf rdf:resource="http://rdaregistry.info/Elements/p/P70017" />
  <rdakit:hasElementType xml:lang="">2</rdakit:hasElementType>
  <reg:hasSubproperty rdf:resource="http://rdaregistry.info/Elements/p/datatype/P70054" />
  <reg:hasSubproperty rdf:resource="http://rdaregistry.info/Elements/p/object/P70054" />
  <reg:hasUnconstrained rdf:resource="http://rdaregistry.info/Elements/u/P60215" />
</rdf:Description>

<!-- Property: is place of birth of -->
<rdf:Description rdf:about="http://rdaregistry.info/Elements/p/P70025">
  <rdfs:isDefinedBy rdf:resource="http://rdaregistry.info/Elements/p/" />
  <reg:status rdf:resource="http://metadataregistry.org/uri/RegStatus/1001" />
  <rdf:type rdf:resource="http://www.w3.org/1999/02/22-rdf-syntax-ns#Property" />
  <reg:name xml:lang="en">placeOfBirthOf</reg:name>
  <rdfs:label xml:lang="en">is place of birth of</rdfs:label>
  <reg:lexicalAlias rdf:resource="http://rdaregistry.info/Elements/p/placeOfBirthOf.en" />
  <rdfs:domain rdf:resource="http://rdaregistry.info/Elements/c/C10009" />
  <rdakit:toolkitLabel xml:lang="en">place of birth of</rdakit:toolkitLabel>
  <reg:hasSubproperty rdf:resource="http://rdaregistry.info/Elements/p/object/P70025" />
  <skos:definition xml:lang="en">Relates a place to a person who was born in a place.</skos:definition>
  <rdakit:toolkitDefinition xml:lang="en">A person who was born in a place.</rdakit:toolkitDefinition>
  <rdfs:subPropertyOf rdf:resource="http://rdaregistry.info/Elements/p/P70014" />
  <rdakit:hasElementType xml:lang="">2</rdakit:hasElementType>
  <reg:hasUnconstrained rdf:resource="http://rdaregistry.info/Elements/u/P60965" />
  <reg:hasSubproperty rdf:resource="http://rdaregistry.info/Elements/p/datatype/P70025" />
</rdf:Description>

<!-- Property: is place of capture of -->
<rdf:Description rdf:about="http://rdaregistry.info/Elements/p/P70038">
  <rdfs:isDefinedBy rdf:resource="http://rdaregistry.info/Elements/p/" />
  <reg:status rdf:resource="http://metadataregistry.org/uri/RegStatus/1001" />
  <rdf:type rdf:resource="http://www.w3.org/1999/02/22-rdf-syntax-ns#Property" />
  <reg:name xml:lang="en">placeOfCaptureOf</reg:name>
  <rdfs:label xml:lang="en">is place of capture of</rdfs:label>
  <reg:lexicalAlias rdf:resource="http://rdaregistry.info/Elements/p/placeOfCaptureOf.en" />
  <rdfs:domain rdf:resource="http://rdaregistry.info/Elements/c/C10009" />
  <rdakit:toolkitLabel xml:lang="en">place of capture of</rdakit:toolkitLabel>
  <reg:hasSubproperty rdf:resource="http://rdaregistry.info/Elements/p/object/P70038" />
  <skos:definition xml:lang="en">Relates a place to an expression that has content that is recorded, filmed, etc., in a place.</skos:definition>
  <rdakit:toolkitDefinition xml:lang="en">An expression that has content that is recorded, filmed, etc., in a place.</rdakit:toolkitDefinition>
  <rdfs:subPropertyOf rdf:resource="http://rdaregistry.info/Elements/p/P70005" />
  <rdakit:hasElementType xml:lang="">2</rdakit:hasElementType>
  <reg:hasUnconstrained rdf:resource="http://rdaregistry.info/Elements/u/P60966" />
  <reg:hasSubproperty rdf:resource="http://rdaregistry.info/Elements/p/datatype/P70038" />
</rdf:Description>

<!-- Property: is place of capture of representative expression of -->
<rdf:Description rdf:about="http://rdaregistry.info/Elements/p/P70052">
  <rdfs:isDefinedBy rdf:resource="http://rdaregistry.info/Elements/p/" />
  <reg:status rdf:resource="http://metadataregistry.org/uri/RegStatus/1001" />
  <rdfs:label xml:lang="en">is place of capture of representative expression of</rdfs:label>
  <rdf:type rdf:resource="http://www.w3.org/1999/02/22-rdf-syntax-ns#Property" />
  <reg:name xml:lang="en">placeOfCaptureOfRepresentativeExpressionOf</reg:name>
  <reg:lexicalAlias rdf:resource="http://rdaregistry.info/Elements/p/placeOfCaptureOfRepresentativeExpressionOf.en" />
  <rdfs:domain rdf:resource="http://rdaregistry.info/Elements/c/C10009" />
  <rdakit:toolkitLabel xml:lang="en">place of capture of representative expression of</rdakit:toolkitLabel>
  <rdakit:hasElementType xml:lang="">2</rdakit:hasElementType>
  <skos:definition xml:lang="en">Relates a place to a work that has content of a representative expression that is recorded, filmed, etc., in a place.</skos:definition>
  <rdakit:toolkitDefinition xml:lang="en">A work that has content of a representative expression that is recorded, filmed, etc., in a place.</rdakit:toolkitDefinition>
  <reg:hasUnconstrained rdf:resource="http://rdaregistry.info/Elements/u/P60966" />
  <reg:hasSubproperty rdf:resource="http://rdaregistry.info/Elements/p/datatype/P70052" />
  <rdfs:subPropertyOf rdf:resource="http://rdaregistry.info/Elements/p/P70004" />
</rdf:Description>

<!-- Property: is place of conference of -->
<rdf:Description rdf:about="http://rdaregistry.info/Elements/p/P70028">
  <rdfs:isDefinedBy rdf:resource="http://rdaregistry.info/Elements/p/" />
  <reg:status rdf:resource="http://metadataregistry.org/uri/RegStatus/1001" />
  <rdf:type rdf:resource="http://www.w3.org/1999/02/22-rdf-syntax-ns#Property" />
  <reg:name xml:lang="en">placeOfConferenceOf</reg:name>
  <rdfs:label xml:lang="en">is place of conference of</rdfs:label>
  <reg:lexicalAlias rdf:resource="http://rdaregistry.info/Elements/p/placeOfConferenceOf.en" />
  <rdfs:domain rdf:resource="http://rdaregistry.info/Elements/c/C10009" />
  <rdakit:toolkitLabel xml:lang="en">place of conference of</rdakit:toolkitLabel>
  <reg:hasSubproperty rdf:resource="http://rdaregistry.info/Elements/p/object/P70028" />
  <rdfs:subPropertyOf rdf:resource="http://rdaregistry.info/Elements/p/P70016" />
  <rdakit:hasElementType xml:lang="">2</rdakit:hasElementType>
  <skos:definition xml:lang="en">Relates a place to a conference, exhibition, or other formally named and convened event that gives rise to a work.</skos:definition>
  <rdakit:toolkitDefinition xml:lang="en">A conference, exhibition, or other formally named and convened event that gives rise to a work.</rdakit:toolkitDefinition>
  <reg:hasSubproperty rdf:resource="http://rdaregistry.info/Elements/p/datatype/P70028" />
  <reg:hasUnconstrained rdf:resource="http://rdaregistry.info/Elements/u/P60997" />
  <skos:altLabel xml:lang="en">location of conference, etc. of</skos:altLabel>
</rdf:Description>

<!-- Property: is place of death of -->
<rdf:Description rdf:about="http://rdaregistry.info/Elements/p/P70026">
  <rdfs:isDefinedBy rdf:resource="http://rdaregistry.info/Elements/p/" />
  <reg:status rdf:resource="http://metadataregistry.org/uri/RegStatus/1001" />
  <rdf:type rdf:resource="http://www.w3.org/1999/02/22-rdf-syntax-ns#Property" />
  <reg:name xml:lang="en">placeOfDeathOf</reg:name>
  <rdfs:label xml:lang="en">is place of death of</rdfs:label>
  <reg:lexicalAlias rdf:resource="http://rdaregistry.info/Elements/p/placeOfDeathOf.en" />
  <rdfs:domain rdf:resource="http://rdaregistry.info/Elements/c/C10009" />
  <rdakit:toolkitLabel xml:lang="en">place of death of</rdakit:toolkitLabel>
  <reg:hasSubproperty rdf:resource="http://rdaregistry.info/Elements/p/object/P70026" />
  <skos:definition xml:lang="en">Relates a place to a person who died in a place.</skos:definition>
  <rdakit:toolkitDefinition xml:lang="en">A person who died in a place.</rdakit:toolkitDefinition>
  <rdfs:subPropertyOf rdf:resource="http://rdaregistry.info/Elements/p/P70014" />
  <rdakit:hasElementType xml:lang="">2</rdakit:hasElementType>
  <reg:hasUnconstrained rdf:resource="http://rdaregistry.info/Elements/u/P60967" />
  <reg:hasSubproperty rdf:resource="http://rdaregistry.info/Elements/p/datatype/P70026" />
</rdf:Description>

<!-- Property: is place of distribution of -->
<rdf:Description rdf:about="http://rdaregistry.info/Elements/p/P70039">
  <rdfs:isDefinedBy rdf:resource="http://rdaregistry.info/Elements/p/" />
  <reg:status rdf:resource="http://metadataregistry.org/uri/RegStatus/1001" />
  <rdf:type rdf:resource="http://www.w3.org/1999/02/22-rdf-syntax-ns#Property" />
  <reg:name xml:lang="en">placeOfDistributionOf</reg:name>
  <rdfs:label xml:lang="en">is place of distribution of</rdfs:label>
  <reg:lexicalAlias rdf:resource="http://rdaregistry.info/Elements/p/placeOfDistributionOf.en" />
  <rdfs:domain rdf:resource="http://rdaregistry.info/Elements/c/C10009" />
  <rdakit:toolkitLabel xml:lang="en">place of distribution of</rdakit:toolkitLabel>
  <reg:hasSubproperty rdf:resource="http://rdaregistry.info/Elements/p/object/P70039" />
  <skos:definition xml:lang="en">Relates a place to a manifestation that is a published manifestation that is distributed from a place.</skos:definition>
  <rdakit:toolkitDefinition xml:lang="en">A manifestation that is a published manifestation that is distributed from a place.</rdakit:toolkitDefinition>
  <rdfs:subPropertyOf rdf:resource="http://rdaregistry.info/Elements/p/P70021" />
  <rdakit:hasElementType xml:lang="">2</rdakit:hasElementType>
  <reg:hasUnconstrained rdf:resource="http://rdaregistry.info/Elements/u/P60968" />
  <reg:hasSubproperty rdf:resource="http://rdaregistry.info/Elements/p/datatype/P70039" />
  <reg:hasSubproperty rdf:resource="http://rdaregistry.info/Elements/p/P70047" />
  <reg:hasSubproperty rdf:resource="http://rdaregistry.info/Elements/p/P70047" />
</rdf:Description>

<!-- Property: is place of manifestation of -->
<rdf:Description rdf:about="http://rdaregistry.info/Elements/p/P70021">
  <rdfs:isDefinedBy rdf:resource="http://rdaregistry.info/Elements/p/" />
  <reg:status rdf:resource="http://metadataregistry.org/uri/RegStatus/1001" />
  <rdf:type rdf:resource="http://www.w3.org/1999/02/22-rdf-syntax-ns#Property" />
  <reg:name xml:lang="en">placeOfManifestationOf</reg:name>
  <rdfs:label xml:lang="en">is place of manifestation of</rdfs:label>
  <reg:lexicalAlias rdf:resource="http://rdaregistry.info/Elements/p/placeOfManifestationOf.en" />
  <rdfs:domain rdf:resource="http://rdaregistry.info/Elements/c/C10009" />
  <rdakit:toolkitLabel xml:lang="en">place of manifestation of</rdakit:toolkitLabel>
  <reg:hasSubproperty rdf:resource="http://rdaregistry.info/Elements/p/object/P70021" />
  <skos:definition xml:lang="en">Relates a place to a manifestation that is a published manifestation that is distributed, printed, duplicated, cast, published, released, or issued, etc., or an unpublished manifestation that is inscribed, fabricated, constructed, etc., in a place.</skos:definition>
  <rdakit:toolkitDefinition xml:lang="en">A manifestation that is a published manifestation that is distributed, printed, duplicated, cast, published, released, or issued, etc., or an unpublished manifestation that is inscribed, fabricated, constructed, etc., in a place.</rdakit:toolkitDefinition>
  <rdfs:subPropertyOf rdf:resource="http://rdaregistry.info/Elements/p/P70006" />
  <rdakit:hasElementType xml:lang="">2</rdakit:hasElementType>
  <reg:hasSubproperty rdf:resource="http://rdaregistry.info/Elements/p/datatype/P70021" />
  <reg:hasSubproperty rdf:resource="http://rdaregistry.info/Elements/p/P70039" />
  <reg:hasSubproperty rdf:resource="http://rdaregistry.info/Elements/p/P70040" />
  <reg:hasSubproperty rdf:resource="http://rdaregistry.info/Elements/p/P70041" />
  <reg:hasSubproperty rdf:resource="http://rdaregistry.info/Elements/p/P70042" />
</rdf:Description>

<!-- Property: is place of manufacture of -->
<rdf:Description rdf:about="http://rdaregistry.info/Elements/p/P70040">
  <rdfs:isDefinedBy rdf:resource="http://rdaregistry.info/Elements/p/" />
  <reg:status rdf:resource="http://metadataregistry.org/uri/RegStatus/1001" />
  <rdf:type rdf:resource="http://www.w3.org/1999/02/22-rdf-syntax-ns#Property" />
  <reg:name xml:lang="en">placeOfManufactureOf</reg:name>
  <rdfs:label xml:lang="en">is place of manufacture of</rdfs:label>
  <reg:lexicalAlias rdf:resource="http://rdaregistry.info/Elements/p/placeOfManufactureOf.en" />
  <rdfs:domain rdf:resource="http://rdaregistry.info/Elements/c/C10009" />
  <rdakit:toolkitLabel xml:lang="en">place of manufacture of</rdakit:toolkitLabel>
  <reg:hasSubproperty rdf:resource="http://rdaregistry.info/Elements/p/object/P70040" />
  <skos:definition xml:lang="en">Relates a place to a manifestation that is a published manifestation that is printed, duplicated, cast, etc., in a place.</skos:definition>
  <rdakit:toolkitDefinition xml:lang="en">A manifestation that is a published manifestation that is printed, duplicated, cast, etc., in a place.</rdakit:toolkitDefinition>
  <rdfs:subPropertyOf rdf:resource="http://rdaregistry.info/Elements/p/P70021" />
  <rdakit:hasElementType xml:lang="">2</rdakit:hasElementType>
  <reg:hasUnconstrained rdf:resource="http://rdaregistry.info/Elements/u/P60969" />
  <reg:hasSubproperty rdf:resource="http://rdaregistry.info/Elements/p/datatype/P70040" />
  <reg:hasSubproperty rdf:resource="http://rdaregistry.info/Elements/p/P70048" />
  <reg:hasSubproperty rdf:resource="http://rdaregistry.info/Elements/p/P70048" />
</rdf:Description>

<!-- Property: is place of origin of work of -->
<rdf:Description rdf:about="http://rdaregistry.info/Elements/p/P70035">
  <rdfs:isDefinedBy rdf:resource="http://rdaregistry.info/Elements/p/" />
  <reg:status rdf:resource="http://metadataregistry.org/uri/RegStatus/1001" />
  <rdf:type rdf:resource="http://www.w3.org/1999/02/22-rdf-syntax-ns#Property" />
  <reg:name xml:lang="en">placeOfOriginOfWorkOf</reg:name>
  <rdfs:label xml:lang="en">is place of origin of work of</rdfs:label>
  <reg:lexicalAlias rdf:resource="http://rdaregistry.info/Elements/p/placeOfOriginOfWorkOf.en" />
  <rdfs:domain rdf:resource="http://rdaregistry.info/Elements/c/C10009" />
  <rdakit:toolkitLabel xml:lang="en">place of origin of work of</rdakit:toolkitLabel>
  <reg:hasSubproperty rdf:resource="http://rdaregistry.info/Elements/p/object/P70035" />
  <skos:definition xml:lang="en">Relates a place to a work which originated from a place.</skos:definition>
  <rdakit:toolkitDefinition xml:lang="en">A work which originated from a place.</rdakit:toolkitDefinition>
  <rdfs:subPropertyOf rdf:resource="http://rdaregistry.info/Elements/p/P70004" />
  <rdakit:hasElementType xml:lang="">2</rdakit:hasElementType>
  <reg:hasUnconstrained rdf:resource="http://rdaregistry.info/Elements/u/P60970" />
  <reg:hasSubproperty rdf:resource="http://rdaregistry.info/Elements/p/datatype/P70035" />
</rdf:Description>

<!-- Property: is place of production of -->
<rdf:Description rdf:about="http://rdaregistry.info/Elements/p/P70041">
  <rdfs:isDefinedBy rdf:resource="http://rdaregistry.info/Elements/p/" />
  <reg:status rdf:resource="http://metadataregistry.org/uri/RegStatus/1001" />
  <rdf:type rdf:resource="http://www.w3.org/1999/02/22-rdf-syntax-ns#Property" />
  <reg:name xml:lang="en">placeOfProductionOf</reg:name>
  <rdfs:label xml:lang="en">is place of production of</rdfs:label>
  <reg:lexicalAlias rdf:resource="http://rdaregistry.info/Elements/p/placeOfProductionOf.en" />
  <rdfs:domain rdf:resource="http://rdaregistry.info/Elements/c/C10009" />
  <rdakit:toolkitLabel xml:lang="en">place of production of</rdakit:toolkitLabel>
  <reg:hasSubproperty rdf:resource="http://rdaregistry.info/Elements/p/object/P70041" />
  <skos:definition xml:lang="en">Relates a place to a manifestation that is an unpublished manifestation that is inscribed, fabricated, constructed, etc., in a place.</skos:definition>
  <rdakit:toolkitDefinition xml:lang="en">A manifestation that is an unpublished manifestation that is inscribed, fabricated, constructed, etc., in a place.</rdakit:toolkitDefinition>
  <rdfs:subPropertyOf rdf:resource="http://rdaregistry.info/Elements/p/P70021" />
  <rdakit:hasElementType xml:lang="">2</rdakit:hasElementType>
  <reg:hasUnconstrained rdf:resource="http://rdaregistry.info/Elements/u/P60971" />
  <reg:hasSubproperty rdf:resource="http://rdaregistry.info/Elements/p/datatype/P70041" />
  <reg:hasSubproperty rdf:resource="http://rdaregistry.info/Elements/p/P70049" />
  <reg:hasSubproperty rdf:resource="http://rdaregistry.info/Elements/p/P70049" />
</rdf:Description>

<!-- Property: is place of publication of -->
<rdf:Description rdf:about="http://rdaregistry.info/Elements/p/P70042">
  <rdfs:isDefinedBy rdf:resource="http://rdaregistry.info/Elements/p/" />
  <reg:status rdf:resource="http://metadataregistry.org/uri/RegStatus/1001" />
  <rdf:type rdf:resource="http://www.w3.org/1999/02/22-rdf-syntax-ns#Property" />
  <reg:name xml:lang="en">placeOfPublicationOf</reg:name>
  <rdfs:label xml:lang="en">is place of publication of</rdfs:label>
  <reg:lexicalAlias rdf:resource="http://rdaregistry.info/Elements/p/placeOfPublicationOf.en" />
  <rdfs:domain rdf:resource="http://rdaregistry.info/Elements/c/C10009" />
  <rdakit:toolkitLabel xml:lang="en">place of publication of</rdakit:toolkitLabel>
  <reg:hasSubproperty rdf:resource="http://rdaregistry.info/Elements/p/object/P70042" />
  <skos:definition xml:lang="en">Relates a place to a manifestation that is a published manifestation that is published, released, or issued in a place.</skos:definition>
  <rdakit:toolkitDefinition xml:lang="en">A manifestation that is a published manifestation that is published, released, or issued in a place.</rdakit:toolkitDefinition>
  <rdfs:subPropertyOf rdf:resource="http://rdaregistry.info/Elements/p/P70021" />
  <rdakit:hasElementType xml:lang="">2</rdakit:hasElementType>
  <reg:hasUnconstrained rdf:resource="http://rdaregistry.info/Elements/u/P60972" />
  <reg:hasSubproperty rdf:resource="http://rdaregistry.info/Elements/p/datatype/P70042" />
  <reg:hasSubproperty rdf:resource="http://rdaregistry.info/Elements/p/P70050" />
  <reg:hasSubproperty rdf:resource="http://rdaregistry.info/Elements/p/P70050" />
</rdf:Description>

<!-- Property: is place of residence of -->
<rdf:Description rdf:about="http://rdaregistry.info/Elements/p/P70027">
  <rdfs:isDefinedBy rdf:resource="http://rdaregistry.info/Elements/p/" />
  <reg:status rdf:resource="http://metadataregistry.org/uri/RegStatus/1001" />
  <rdf:type rdf:resource="http://www.w3.org/1999/02/22-rdf-syntax-ns#Property" />
  <reg:name xml:lang="en">placeOfResidenceOf</reg:name>
  <rdfs:label xml:lang="en">is place of residence of</rdfs:label>
  <reg:lexicalAlias rdf:resource="http://rdaregistry.info/Elements/p/placeOfResidenceOf.en" />
  <rdfs:domain rdf:resource="http://rdaregistry.info/Elements/c/C10009" />
  <rdakit:toolkitLabel xml:lang="en">place of residence of</rdakit:toolkitLabel>
  <reg:hasSubproperty rdf:resource="http://rdaregistry.info/Elements/p/object/P70027" />
  <skos:definition xml:lang="en">Relates a place to a person who resides or has resided in a place.</skos:definition>
  <rdakit:toolkitDefinition xml:lang="en">A person who resides or has resided in a place.</rdakit:toolkitDefinition>
  <rdfs:subPropertyOf rdf:resource="http://rdaregistry.info/Elements/p/P70014" />
  <rdakit:hasElementType xml:lang="">2</rdakit:hasElementType>
  <reg:hasUnconstrained rdf:resource="http://rdaregistry.info/Elements/u/P60973" />
  <reg:hasSubproperty rdf:resource="http://rdaregistry.info/Elements/p/datatype/P70027" />
</rdf:Description>

<!-- Property: has related entity of place -->
<rdf:Description rdf:about="http://rdaregistry.info/Elements/p/P70053">
  <rdfs:isDefinedBy rdf:resource="http://rdaregistry.info/Elements/p/" />
  <reg:status rdf:resource="http://metadataregistry.org/uri/RegStatus/1001" />
  <rdfs:label xml:lang="en">has related entity of place</rdfs:label>
  <reg:lexicalAlias rdf:resource="http://rdaregistry.info/Elements/p/relatedEntityOfPlace.en" />
  <skos:definition xml:lang="en">Relates a place to an entity that is associated with a place.</skos:definition>
  <rdakit:toolkitLabel xml:lang="en">related entity of place</rdakit:toolkitLabel>
  <rdakit:toolkitDefinition xml:lang="en">An entity that is associated with a place.</rdakit:toolkitDefinition>
  <rdf:type rdf:resource="http://www.w3.org/1999/02/22-rdf-syntax-ns#Property" />
  <reg:name xml:lang="">relatedEntityOfPlace</reg:name>
  <rdfs:domain rdf:resource="http://rdaregistry.info/Elements/c/C10009" />
  <rdakit:hasElementType xml:lang="">1</rdakit:hasElementType>
  <rdfs:subPropertyOf rdf:resource="http://rdaregistry.info/Elements/x/P00028" />
  <reg:hasUnconstrained rdf:resource="http://rdaregistry.info/Elements/u/P61036" />
</rdf:Description>

<!-- Property: has related RDA entity of place -->
<rdf:Description rdf:about="http://rdaregistry.info/Elements/p/P70013">
  <rdfs:isDefinedBy rdf:resource="http://rdaregistry.info/Elements/p/" />
  <reg:status rdf:resource="http://metadataregistry.org/uri/RegStatus/1001" />
  <rdf:type rdf:resource="http://www.w3.org/1999/02/22-rdf-syntax-ns#Property" />
  <reg:name xml:lang="en">relatedRDAEntityOfPlace</reg:name>
  <rdfs:label xml:lang="en">has related RDA entity of place</rdfs:label>
  <reg:lexicalAlias rdf:resource="http://rdaregistry.info/Elements/p/relatedRDAEntityOfPlace.en" />
  <skos:definition xml:lang="en">Relates a place to an RDA entity that is associated with a place.</skos:definition>
  <rdfs:domain rdf:resource="http://rdaregistry.info/Elements/c/C10009" />
  <reg:hasSubproperty rdf:resource="http://rdaregistry.info/Elements/p/datatype/P70013" />
  <reg:hasSubproperty rdf:resource="http://rdaregistry.info/Elements/p/P70004" />
  <reg:hasSubproperty rdf:resource="http://rdaregistry.info/Elements/p/P70005" />
  <reg:hasSubproperty rdf:resource="http://rdaregistry.info/Elements/p/P70006" />
  <reg:hasSubproperty rdf:resource="http://rdaregistry.info/Elements/p/P70007" />
  <reg:hasSubproperty rdf:resource="http://rdaregistry.info/Elements/p/P70008" />
  <reg:hasSubproperty rdf:resource="http://rdaregistry.info/Elements/p/P70010" />
  <reg:hasSubproperty rdf:resource="http://rdaregistry.info/Elements/p/P70011" />
  <reg:hasSubproperty rdf:resource="http://rdaregistry.info/Elements/p/P70012" />
  <reg:name xml:lang="da">relateretEntitetSted</reg:name>
  <rdfs:label xml:lang="da">har relateret entitet (sted)</rdfs:label>
  <reg:lexicalAlias rdf:resource="http://rdaregistry.info/Elements/p/relateretEntitetSted.da" />
  <skos:definition xml:lang="da">Relaterer et sted til en entitet der er knyttet til et beskrevet sted.</skos:definition>
  <reg:name xml:lang="vi">địaĐiểmThựcThểCóLiênQuan</reg:name>
  <rdfs:label xml:lang="vi">có thực thể có liên quan (địa điểm)</rdfs:label>
  <skos:definition xml:lang="vi">Liên kết địa điểm với thực thể liên quan tới địa điểm đang được mô tả.</skos:definition>
  <rdfs:label xml:lang="ca">té com a entitat relacionada (lloc)</rdfs:label>
  <skos:definition xml:lang="ca">Relaciona un lloc amb una entitat associada amb un lloc que es descriu.</skos:definition>
  <reg:name xml:lang="fi">paikkaanLiittyvaEntiteetti</reg:name>
  <rdfs:label xml:lang="fi">paikkaan liittyvä entiteetti</rdfs:label>
  <reg:lexicalAlias rdf:resource="http://rdaregistry.info/Elements/p/paikkaanLiittyvaEntiteetti.fi" />
  <skos:definition xml:lang="fi">Liittää paikan entiteettiin, johon kuvailun kohteena oleva paikka liittyy.</skos:definition>
  <reg:name xml:lang="fr">entitéEnRelationLieu</reg:name>
  <rdfs:label xml:lang="fr">a pour entité en relation (lieu)</rdfs:label>
  <reg:lexicalAlias rdf:resource="http://rdaregistry.info/Elements/p/entitéEnRelationLieu.fr" />
  <skos:definition xml:lang="fr">Met un lieu en relation avec une entité associée à un lieu décrit.</skos:definition>
  <reg:name xml:lang="el">σχετικήΟντότηταΤόπος</reg:name>
  <rdfs:label xml:lang="el">έχει σχετική οντότητα (τόπος)</rdfs:label>
  <reg:lexicalAlias rdf:resource="http://rdaregistry.info/Elements/p/σχετικήΟντότηταΤόπος.el" />
  <skos:definition xml:lang="el">Συνδέει έναν τόπο με μια οντότητα που συνδέεται με έναν περιγραφόμενο τόπο.</skos:definition>
  <rdakit:toolkitLabel xml:lang="en">related RDA entity of place</rdakit:toolkitLabel>
  <rdakit:toolkitDefinition xml:lang="en">An RDA entity that is associated with a place.</rdakit:toolkitDefinition>
  <rdakit:hasElementType xml:lang="">1</rdakit:hasElementType>
  <rdfs:subPropertyOf rdf:resource="http://rdaregistry.info/Elements/p/P70053" />
  <reg:name xml:lang="hu">kapcsolódóEntitásHely</reg:name>
  <rdfs:label xml:lang="hu">van kapcsolódó entitása (hely)</rdfs:label>
  <skos:definition xml:lang="hu">Egy helyet hozzákapcsol egy entitáshoz, amely kötődik egy éppen leírt helyhez.</skos:definition>
  <rdfs:subPropertyOf rdf:resource="http://rdaregistry.info/Elements/x/P00001" />
  <reg:hasUnconstrained rdf:resource="http://rdaregistry.info/Elements/u/P61036" />
</rdf:Description>

<!-- Property: is right ascension and declination of -->
<rdf:Description rdf:about="http://rdaregistry.info/Elements/p/P70036">
  <rdfs:isDefinedBy rdf:resource="http://rdaregistry.info/Elements/p/" />
  <reg:status rdf:resource="http://metadataregistry.org/uri/RegStatus/1001" />
  <rdf:type rdf:resource="http://www.w3.org/1999/02/22-rdf-syntax-ns#Property" />
  <reg:name xml:lang="en">rightAscensionAndDeclinationOf</reg:name>
  <rdfs:label xml:lang="en">is right ascension and declination of</rdfs:label>
  <reg:lexicalAlias rdf:resource="http://rdaregistry.info/Elements/p/rightAscensionAndDeclinationOf.en" />
  <rdfs:domain rdf:resource="http://rdaregistry.info/Elements/c/C10009" />
  <rdakit:toolkitLabel xml:lang="en">right ascension and declination of</rdakit:toolkitLabel>
  <reg:hasSubproperty rdf:resource="http://rdaregistry.info/Elements/p/object/P70036" />
  <rdfs:subPropertyOf rdf:resource="http://rdaregistry.info/Elements/p/P70023" />
  <rdakit:hasElementType xml:lang="">2</rdakit:hasElementType>
  <reg:hasSubproperty rdf:resource="http://rdaregistry.info/Elements/p/datatype/P70036" />
  <skos:definition xml:lang="en">Relates a place to a work that is a cartographic work that locates a celestial body that is the coverage of the work and is identified using the angles of right ascension and declination.</skos:definition>
  <rdakit:toolkitDefinition xml:lang="en">A work that is a cartographic work that locates a celestial body that is the coverage of the work and is identified using the angles of right ascension and declination.</rdakit:toolkitDefinition>
</rdf:Description>

<!-- Property: is strings of coordinate pairs of -->
<rdf:Description rdf:about="http://rdaregistry.info/Elements/p/P70037">
  <rdfs:isDefinedBy rdf:resource="http://rdaregistry.info/Elements/p/" />
  <reg:status rdf:resource="http://metadataregistry.org/uri/RegStatus/1001" />
  <rdf:type rdf:resource="http://www.w3.org/1999/02/22-rdf-syntax-ns#Property" />
  <reg:name xml:lang="en">stringsOfCoordinatePairsOf</reg:name>
  <rdfs:label xml:lang="en">is strings of coordinate pairs of</rdfs:label>
  <reg:lexicalAlias rdf:resource="http://rdaregistry.info/Elements/p/stringsOfCoordinatePairsOf.en" />
  <rdfs:domain rdf:resource="http://rdaregistry.info/Elements/c/C10009" />
  <rdakit:toolkitLabel xml:lang="en">strings of coordinate pairs of</rdakit:toolkitLabel>
  <reg:hasSubproperty rdf:resource="http://rdaregistry.info/Elements/p/object/P70037" />
  <rdfs:subPropertyOf rdf:resource="http://rdaregistry.info/Elements/p/P70023" />
  <rdakit:hasElementType xml:lang="">2</rdakit:hasElementType>
  <reg:hasSubproperty rdf:resource="http://rdaregistry.info/Elements/p/datatype/P70037" />
  <skos:definition xml:lang="en">Relates a place to a work that is a cartographic work that has an area of coverage that is identifiedy by a polygon using coordinates for each vertex.</skos:definition>
  <rdakit:toolkitDefinition xml:lang="en">A work that is a cartographicwork  that has an area of coverage that is identifiedy by a polygon using coordinates for each vertex.</rdakit:toolkitDefinition>
</rdf:Description>

<!-- Property: has variant access point for place -->
<rdf:Description rdf:about="http://rdaregistry.info/Elements/p/P70046">
  <rdfs:isDefinedBy rdf:resource="http://rdaregistry.info/Elements/p/" />
  <reg:status rdf:resource="http://metadataregistry.org/uri/RegStatus/1001" />
  <rdf:type rdf:resource="http://www.w3.org/1999/02/22-rdf-syntax-ns#Property" />
  <reg:name xml:lang="en">variantAccessPointForPlace</reg:name>
  <rdfs:label xml:lang="en">has variant access point for place</rdfs:label>
  <reg:lexicalAlias rdf:resource="http://rdaregistry.info/Elements/p/variantAccessPointForPlace.en" />
  <skos:definition xml:lang="en">Relates a place to an access point of place that is not selected for preference in a specific vocabulary encoding scheme.</skos:definition>
  <rdfs:domain rdf:resource="http://rdaregistry.info/Elements/c/C10009" />
  <rdakit:toolkitLabel xml:lang="en">variant access point for place</rdakit:toolkitLabel>
  <rdakit:toolkitDefinition xml:lang="en">An access point of place that is not selected for preference in a specific vocabulary encoding scheme.</rdakit:toolkitDefinition>
  <reg:hasUnconstrained rdf:resource="http://rdaregistry.info/Elements/u/P60917" />
  <reg:hasSubproperty rdf:resource="http://rdaregistry.info/Elements/p/object/P70046" />
  <rdfs:subPropertyOf rdf:resource="http://rdaregistry.info/Elements/p/P70018" />
  <rdakit:hasElementType xml:lang="">3</rdakit:hasElementType>
  <reg:hasSubproperty rdf:resource="http://rdaregistry.info/Elements/p/datatype/P70046" />
  <rdfs:subPropertyOf rdf:resource="http://rdaregistry.info/Elements/x/P00022" />
</rdf:Description>


<!-- Status properties used in this document  -->
    <skos:Concept rdf:about="http://metadataregistry.org/uri/RegStatus/1001">
        <skos:prefLabel xml:lang="en">Published</skos:prefLabel>
    </skos:Concept>
    <skos:Concept rdf:about="http://metadataregistry.org/uri/RegStatus/1008">
        <skos:prefLabel xml:lang="en">Deprecated</skos:prefLabel>
    </skos:Concept>
</rdf:RDF>
