<?xml version="1.0" encoding="UTF-8" ?>                       
<?xml-stylesheet type="text/xsl" href="ontology.xsl" ?>
<rdf:RDF
  xml:base="http://lexvo.org/ontology"
  xmlns:lvont="http://lexvo.org/ontology"
  xmlns:rdf="http://www.w3.org/1999/02/22-rdf-syntax-ns#"
  xmlns:rdfs="http://www.w3.org/2000/01/rdf-schema#"
  xmlns:owl="http://www.w3.org/2002/07/owl#"
  xmlns:xsd="http://www.w3.org/2001/XMLSchema#"
  xmlns:dcterms="http://purl.org/dc/terms/"
  xmlns:skos="http://www.w3.org/2004/02/skos/core#"
  xmlns:foaf="http://xmlns.com/foaf/0.1/" >

<!--

Lexvo.org Ontology Version 0.22 (2013-05-24)
Gerard de Melo, 2010-2012
http://www.lexvo.org/
http://lexvo.org/ontology

Note: The Lexvo.org ontology is still under development and may not be able to address all
needs. Please also consider using the Lingvoj Ontology and the GOLD ontology, whereever
appropriate.
http://www.lingvoj.org/ontology
http://www.linguistics-ontology.org/gold.html

-->

<owl:Ontology rdf:about="">
  <rdfs:comment>Lexvo.org Ontology</rdfs:comment>
  <rdfs:label xml:lang="en">Lexvo.org Ontology</rdfs:label>
  <owl:versionInfo xml:lang="en">Lexvo.org Ontology Version 0.22 (2013-05-24)</owl:versionInfo>
  <dcterms:modified rdf:datatype="xsd:date">2013-05-24</dcterms:modified>
  <foaf:homepage rdf:resource="http://www.lexvo.org/" />
  <dcterms:creator rdf:resource="http://www.demelo.org/gdm/#GDM" />
  <dcterms:contributor rdf:resource="http://data.semanticweb.org/person/bernard-vatant" />
  <rdfs:seeAlso rdf:resource="http://www.lexvo.org/" />
  <dcterms:subject rdf:resource="http://dbpedia.org/resource/Language" />
</owl:Ontology>

<owl:Class rdf:about="#Language">
  <rdfs:comment xml:lang="en">Groups of human language variants that are or were spoken, written, or signed at some point in time.</rdfs:comment>
  <skos:note xml:lang="en">This definition includes languages, particular language variants (e.g. dialects), and larger groups of language 
    variants (e.g. macrolanguages and language families), as the distinction between them is largely conventional.</skos:note>
  <rdfs:label xml:lang="en">language</rdfs:label>
  <rdfs:subClassOf rdf:resource="http://purl.org/dc/terms/LinguisticSystem"/>
  <lvont:somewhatSameAs rdf:resource="http://www.lingvoj.org/ontology#Lingvo"/>
  <rdfs:seeAlso rdf:resource="http://en.wikipedia.org/wiki/Language" />
</owl:Class>

<owl:Class rdf:about="#Term">
  <rdfs:comment xml:lang="en">A term in a specific language.</rdfs:comment>
  <rdfs:label xml:lang="en">term</rdfs:label>
  <lvont:subClassOf rdf:resource="http://www.w3.org/2008/05/skos-xl#Label"/>
  <lvont:nearlySameAs rdf:resource="http://lexonto.ontoware.org/lmf#FormRepresentation"/>
</owl:Class>

<owl:Class rdf:about="#Character">
  <rdfs:comment xml:lang="en">An abstract character as defined by the Unicode Standard,
  Version 5, in Chapter 3.4.</rdfs:comment>
  <rdfs:label xml:lang="en">character</rdfs:label>
  <skos:note xml:lang="en">The same abstract character may be rendered in different forms, depending on the language and on typeface characters.</skos:note>
  <owl:sameAs rdf:resource="http://purl.org/linguistics/gold/Character" />
</owl:Class>

<owl:Class rdf:about="#CJKRadical">
  <rdfs:comment xml:lang="en">A CJK character radical.</rdfs:comment>
  <rdfs:label xml:lang="en">radical</rdfs:label>
  <rdfs:seeAlso rdf:resource="http://en.wikipedia.org/wiki/Radical_%28Chinese_character%29" />
  <skos:note xml:lang="en">CJK radicals are slightly more abstract than characters, because the same radical can be manifested as different
    characters, e.g. radical 4 can take the form of '丿', '乀', or '乁'.</skos:note>
</owl:Class>

<owl:Class rdf:about="#Script">
  <rdfs:comment xml:lang="en">A writing system considered abstractly, i.e. independent
    of language-specific variations.</rdfs:comment>
  <rdfs:label xml:lang="en">script</rdfs:label>
</owl:Class>

<owl:Class rdf:about="#GeographicRegion">
  <rdfs:comment xml:lang="en">Geographic regions on Earth or elsewhere.</rdfs:comment>
  <rdfs:label xml:lang="en">geographic region</rdfs:label>
</owl:Class>

<owl:SymmetricProperty rdf:about="#somewhatSameAs">
  <rdfs:comment xml:lang="en">The property of being at least somewhat the same as something else. For instance,
    the City of Los Angeles is somewhat the same as the Greater Los Angeles area.</rdfs:comment>
  <rdfs:label xml:lang="en">somewhat same as</rdfs:label>
  <lvont:somewhatSameAs rdf:resource="http://www.w3.org/2004/02/skos/core#broadMatch" />
</owl:SymmetricProperty>

<rdf:Description rdf:about="http://www.w3.org/2004/02/skos/core#broadMatch">
  <rdfs:subPropertyOf rdf:resource="http://lexvo.org/ontology#somewhatSameAs" />
</rdf:Description>

<owl:SymmetricProperty rdf:about="#nearlySameAs">
  <rdfs:comment xml:lang="en">The property of being at least nearly the same as something else. For instance,
    the geographical area comprising the island of Malta is nearly the same as the island of Malta.</rdfs:comment>
  <rdfs:label xml:lang="en">nearly same as</rdfs:label>
  <rdfs:subPropertyOf rdf:resource="http://lexvo.org/ontology#somewhatSameAs" />
  <lvont:somewhatSameAs rdf:resource="http://www.w3.org/2002/07/owl#sameAs" />
</owl:SymmetricProperty>

<rdf:Description rdf:about="http://www.w3.org/2004/02/skos/core#exactMatch">
  <rdfs:subPropertyOf rdf:resource="http://lexvo.org/ontology#nearlySameAs" />
</rdf:Description>

<rdf:Description rdf:about="http://www.w3.org/2002/07/owl#sameAs">
  <rdfs:subPropertyOf rdf:resource="http://lexvo.org/ontology#nearlySameAs" />
</rdf:Description>

<owl:SymmetricProperty rdf:about="#strictlySameAs">
  <rdfs:comment xml:lang="en">The property of genuine identity in the Leibnizian sense.</rdfs:comment>
  <rdfs:label xml:lang="en">same as</rdfs:label>
  <rdfs:subPropertyOf rdf:resource="http://lexvo.org/ontology#nearlySameAs" />
  <owl:sameAs rdf:resource="http://www.w3.org/2002/07/owl#sameAs" />
</owl:SymmetricProperty>

<owl:ObjectProperty rdf:about="#represents">
  <rdfs:comment xml:lang="en">the semiotic property of semantically representing something, i.e. a
    relationship between words and other signs and resources that they represent (or represented) to a considerable number of humans</rdfs:comment>
  <rdfs:label xml:lang="en">represents</rdfs:label>
</owl:ObjectProperty>

<owl:ObjectProperty rdf:about="#representedBy">
  <owl:inverseOf rdf:resource="http://lexvo.org/ontology#represents"/>
  <rdfs:label xml:lang="en">represented by</rdfs:label>
</owl:ObjectProperty>

<owl:ObjectProperty rdf:about="#means">
  <rdfs:subPropertyOf rdf:resource="http://lexvo.org/ontology#represents" />
  <owl:inverseOf rdf:resource="http://lexvo.org/ontology#label"/>
  <rdfs:comment xml:lang="en">the semiotic property of a natural language word meaning something, i.e. a
    relationship between words and resources that they represent (or represented) to a considerable number of humans</rdfs:comment>
  <rdfs:label xml:lang="en">means</rdfs:label>
</owl:ObjectProperty>

<owl:ObjectProperty rdf:about="#label">
  <rdfs:range rdf:resource="http://www.w3.org/2008/05/skos-xl#Label" />
  <rdfs:subPropertyOf rdf:resource="http://lexvo.org/ontology#representedBy" />
  <owl:inverseOf rdf:resource="http://lexvo.org/ontology#means" />
  <rdfs:comment xml:lang="en">the semiotic property of possessing a natural language label (as opposed to artificial identifiers), e.g. the city of Paris is lexicalized in Italian using the Italian term "Parigi".</rdfs:comment>
  <skos:note xml:lang="en">This property is more general than skosxl:prefLabel and skosxl:altLabel, as it does not make any normative claims about which labels are preferred. It merely describes
    the fact that a certain label can be used to refer to something.</skos:note>
  <rdfs:label xml:lang="en">has label</rdfs:label>
  <!-- property chain axiom, given informally as a comment -->
  <rdfs:comment xml:lang="en">If C lvont:Label L and L skosxl:literalForm V, then X rdfs:label V.</rdfs:comment>
</owl:ObjectProperty>

<rdf:Description rdf:about="http://www.w3.org/2008/05/skos-xl#prefLabel">
  <rdfs:subPropertyOf rdf:resource="http://lexvo.org/ontology#label" />
</rdf:Description>

<rdf:Description rdf:about="http://www.w3.org/2008/05/skos-xl#altLabel">
  <rdfs:subPropertyOf rdf:resource="http://lexvo.org/ontology#label" />
</rdf:Description>

<owl:ObjectProperty rdf:about="#language">
  <rdfs:comment xml:lang="en">The property of a resource being mainly encoded in a specific language.</rdfs:comment>
  <rdfs:range rdf:resource="http://lexvo.org/ontology#Language" />
  <rdfs:label xml:lang="en">in language</rdfs:label>
  <rdfs:subPropertyOf rdf:resource="http://purl.org/dc/elements/1.1/language" />
  <rdfs:subPropertyOf rdf:resource="http://purl.org/dc/terms/language" />
</owl:ObjectProperty>

<owl:ObjectProperty rdf:about="#containsCharacter">
  <rdfs:comment xml:lang="en">The property of a term containing a specific character.</rdfs:comment>
  <rdfs:domain rdf:resource="http://lexvo.org/ontology#Term" />
  <rdfs:range rdf:resource="http://lexvo.org/ontology#Character" />
  <rdfs:label xml:lang="en">contains character</rdfs:label>
</owl:ObjectProperty>

<owl:SymmetricProperty rdf:about="#translation">
  <rdfs:comment xml:lang="en">translational equivalence between words and other signs
    and resources that they represent to or represented to a considerable number of humans</rdfs:comment>
  <rdfs:label xml:lang="en">translation</rdfs:label>
  <lvont:nearlySameAs rdf:resource="http://purl.org/linguistics/gold/translation" />
  <skos:note xml:lang="en">Domain and range are usually Term objects, however string literals are acceptable as well for the range.</skos:note>
</owl:SymmetricProperty>

<owl:ObjectProperty rdf:about="#variant">
  <rdfs:comment xml:lang="en">The property of being a variant of another resource.</rdfs:comment>
  <rdfs:label xml:lang="en">variant</rdfs:label>
  <skos:note xml:lang="en">Especially for terms and characters.</skos:note>
</owl:ObjectProperty>

<owl:DatatypeProperty rdf:about="#iso639P1Code">
  <rdfs:domain rdf:resource="http://lexvo.org/ontology#Language" />
  <rdfs:label xml:lang="en">ISO 639-1 code</rdfs:label>
  <owl:equivalentProperty rdf:resource="http://www.lingvoj.org/ontology#iso1"/>
  <owl:equivalentProperty rdf:resource="http://psi.oasis-open.org/iso/639/#code-a2"/>
</owl:DatatypeProperty>

<owl:DatatypeProperty rdf:about="#iso6392BCode">
  <rdfs:domain rdf:resource="http://lexvo.org/ontology#Language"/>
  <rdfs:label xml:lang="en">ISO 639-2 Bibliographical code</rdfs:label>
  <owl:equivalentProperty rdf:resource="http://www.lingvoj.org/ontology#iso2b"/>
  <owl:equivalentProperty rdf:resource="http://psi.oasis-open.org/iso/639/#code-a3b"/>
  <rdfs:seeAlso rdf:resource="http://www.loc.gov/standards/iso639-2/" />
</owl:DatatypeProperty>

<owl:DatatypeProperty rdf:about="#iso6392TCode">
  <rdfs:domain rdf:resource="http://lexvo.org/ontology#Language"/>
  <rdfs:label xml:lang="en">ISO 639-2 Terminological code</rdfs:label>
  <owl:equivalentProperty rdf:resource="http://www.lingvoj.org/ontology#iso2t"/>
  <owl:equivalentProperty rdf:resource="http://psi.oasis-open.org/iso/639/#code-a3t"/>
  <rdfs:seeAlso rdf:resource="http://www.loc.gov/standards/iso639-2/" />
</owl:DatatypeProperty>

<owl:DatatypeProperty rdf:about="#iso639P3PCode">
  <rdfs:domain rdf:resource="http://lexvo.org/ontology#Language"/>
  <rdfs:label xml:lang="en">ISO 639-3 code</rdfs:label>
  <owl:equivalentProperty rdf:resource="http://www.lingvoj.org/ontology#iso3"/>
  <rdfs:seeAlso rdf:resource="http://www.sil.org/ISO639-3/" />
</owl:DatatypeProperty>

<owl:DatatypeProperty rdf:about="#iso639P5Code">
  <rdfs:domain rdf:resource="http://lexvo.org/ontology#Language"/>
  <rdfs:label xml:lang="en">ISO 639-5 code</rdfs:label>
  <rdfs:seeAlso rdf:resource="http://www.loc.gov/standards/iso639-5/" />
</owl:DatatypeProperty>

<owl:DatatypeProperty rdf:about="#marcCode">
  <rdfs:domain rdf:resource="http://lexvo.org/ontology#Language"/>
  <rdfs:label xml:lang="en">MARC 21 / USMARC code</rdfs:label>
  <rdfs:seeAlso rdf:resource="http://www.loc.gov/marc/" />
</owl:DatatypeProperty>

<owl:DatatypeProperty rdf:about="#iso15924Alphacode">
  <rdfs:domain rdf:resource="http://lexvo.org/ontology#Script"/>
  <rdfs:label xml:lang="en">ISO 15924 alphabetic code</rdfs:label>
  <rdfs:seeAlso rdf:resource="http://unicode.org/iso15924/" />
</owl:DatatypeProperty>

<owl:ObjectProperty rdf:about="#inScript">
  <rdfs:comment xml:lang="en">The property of a document being written in a specific script,
    or a language being written or having being written in a specific script by a considerable
    group of language users.</rdfs:comment>
  <rdfs:label xml:lang="en">in script</rdfs:label>
  <rdfs:range rdf:resource="http://lexvo.org/ontology#Script"/>
</owl:ObjectProperty>

<owl:ObjectProperty rdf:about="#usesScript">
  <rdfs:comment xml:lang="en">The property of a language being written or having being written in a specific 
    script by a considerable group of language users.</rdfs:comment>
  <rdfs:label xml:lang="en">uses script</rdfs:label>
  <owl:inverseOf rdf:resource="http://lexvo.org/ontology#scriptFor" />
  <rdfs:range rdf:resource="http://lexvo.org/ontology#Script"/>
</owl:ObjectProperty>

<owl:ObjectProperty rdf:about="#scriptFor">
  <rdfs:comment xml:lang="en">The property of a script being used for a particular language by
   a considerable of language users (but not necessarily the majority of all language users).</rdfs:comment>
  <rdfs:label xml:lang="en">script for</rdfs:label>
  <owl:inverseOf rdf:resource="http://lexvo.org/ontology#usesScript" />
  <rdfs:domain rdf:resource="http://lexvo.org/ontology#Script"/>
  <rdfs:range rdf:resource="http://lexvo.org/ontology#Language"/>
</owl:ObjectProperty>

<owl:ObjectProperty rdf:about="#usedIn">
  <rdfs:comment xml:lang="en">The property of a language or writing system
    being used somewhat extensively in a particular geographical region 
    at some point in time.</rdfs:comment>
  <rdfs:label xml:lang="en">used in</rdfs:label>
  <rdfs:range rdf:resource="http://lexvo.org/ontology#GeographicRegion"/>
</owl:ObjectProperty>

<owl:ObjectProperty rdf:about="#hasCharacterComponent">
  <rdfs:comment xml:lang="en">The property of a character being composed of another character.</rdfs:comment>
  <rdfs:label xml:lang="en">character component</rdfs:label>
  <rdfs:domain rdf:resource="http://lexvo.org/ontology#Character"/>
  <rdfs:range rdf:resource="http://lexvo.org/ontology#Character"/>
  <skos:note xml:lang="en">Especially for CJK characters.</skos:note>
</owl:ObjectProperty>

<owl:ObjectProperty rdf:about="#characterRadical">
  <rdfs:comment xml:lang="en">The property of a CJK character being conventionally
    associated with a CJK character radical.</rdfs:comment>
  <rdfs:label xml:lang="en">translation</rdfs:label>
  <rdfs:domain rdf:resource="http://lexvo.org/ontology#Character"/>
  <rdfs:range rdf:resource="http://lexvo.org/ontology#CJKRadical"/>
</owl:ObjectProperty>

<owl:DatatypeProperty rdf:about="#nonRadicalStrokes">
  <rdfs:comment xml:lang="en">The property of a character conventionally being
    written with a specific number strokes, excluding the strokes of its radical.</rdfs:comment>
  <rdfs:label xml:lang="en">non-radical strokes</rdfs:label>
  <rdfs:domain rdf:resource="http://lexvo.org/ontology#Character"/>
  <rdfs:range rdf:resource="http://www.w3.org/2001/XMLSchema#nonNegativeInteger"/>
  <skos:note xml:lang="en">Especially for CJK characters.</skos:note>
</owl:DatatypeProperty>

<owl:ObjectProperty rdf:about="#broader">
  <rdfs:comment xml:lang="en">The property of having a broader, more generic concept.</rdfs:comment>
  <rdfs:label xml:lang="en">broader</rdfs:label>
  <owl:inverseOf rdf:resource="http://lexvo.org/ontology#narrower"/>
  <lvont:somewhatSameAs rdf:resource="http://www.w3.org/2004/02/skos/core#broader"/>
  <skos:note xml:lang="en">Similar to skos:broader but domain and range are not restricted to skos:Concept instances.</skos:note>
</owl:ObjectProperty>

<owl:ObjectProperty rdf:about="#narrower">
  <rdfs:comment xml:lang="en">The property of having a narrower, less generic concept.</rdfs:comment>
  <rdfs:label xml:lang="en">narrower</rdfs:label>
  <owl:inverseOf rdf:resource="http://lexvo.org/ontology#broader"/>
  <lvont:somewhatSameAs rdf:resource="http://www.w3.org/2004/02/skos/core#narrower"/>
  <skos:note xml:lang="en">Similar to skos:narrower but domain and range are not restricted to skos:Concept instances.</skos:note>
</owl:ObjectProperty>

<owl:ObjectProperty rdf:about="#memberOf">
  <rdfs:comment xml:lang="en">The property of being a member of a group.</rdfs:comment>
  <rdfs:label xml:lang="en">member of</rdfs:label>
  <owl:inverseOf rdf:resource="http://lexvo.org/ontology#hasMember"/>
  <skos:note xml:lang="en">For instance for geographic regions.</skos:note>
</owl:ObjectProperty>

<owl:ObjectProperty rdf:about="#hasMember">
  <rdfs:comment xml:lang="en">The property of having a member.</rdfs:comment>
  <rdfs:label xml:lang="en">has member</rdfs:label>
  <owl:inverseOf rdf:resource="http://lexvo.org/ontology#memberOf"/>
  <skos:note xml:lang="en">For instance for geographic regions.</skos:note>
</owl:ObjectProperty>

<owl:ObjectProperty rdf:about="#isFocusOf">
  <owl:inverseOf rdf:resource="http://xmlns.com/foaf/0.1/focus"/>
  <rdfs:label xml:lang="en">is focus of</rdfs:label>
  <skos:note xml:lang="en">The isFocusOf relates an entity to relevant SKOS concepts 
    that are conceptualizations of the same entity. This is the inverse of the
    standard foaf:focus property, which connects a SKOS concept to a relevant
    non-conceptualized entity.</skos:note>
</owl:ObjectProperty>

</rdf:RDF>
